Proof of confluence
- Removed the tred_C_elim rule

Lang/Semantics.v
@@ -1,7 +1,7 @@
 Require Import Utf8.
 Require Import Syntax.
 Require Import Typing.
-Require Import Binding.Lib Binding.Env Binding.Product.
+Require Import Binding.Lib Binding.Env Binding.Product Binding.Set.
 Require Import Relation_Operators.
 
 Open Scope bind_scope.
@@ -9,6 +9,7 @@ Open Scope bind_scope.
 Reserved Notation "M '→ₜ' M'" (at level 67).
 Reserved Notation "J '→ⱼ' J'" (at level 67).
 Reserved Notation "V '→ᵥ' V'" (at level 67).
+Reserved Notation "E '→ₑ' E'" (at level 67).
 
 Inductive tred {S : VSig} : term S → term S → Prop :=
   | tred_beta : ∀ M (V : value S),
@@ -17,8 +18,6 @@ Inductive tred {S : VSig} : term S → term S → Prop :=
     t_app (t_ctrl J) N →ₜ t_ctrl (struct_subst J (e_appl e_hole (shift N)))
   | tred_C_R : ∀ J (V : value S),
     t_app V (t_ctrl J) →ₜ t_ctrl (struct_subst J (e_appr (shift V) e_hole))
-  | tred_C_elim : ∀ M,
-    t_ctrl (j_jmp (k_var VZ) (shift M)) →ₜ M
 
   | tred_value : ∀ V V',
     V →ᵥ V' →
@@ -50,10 +49,232 @@ where "M →ₜ M'" := (tred M M')
   and "J →ⱼ J'" := (jred J J')
   and "V →ᵥ V'" := (vred V V').
 
-Notation tred_rtc M₁ M₂ := (clos_trans_1n _ tred M₁ M₂).
-Notation vred_rtc V₁ V₂ := (clos_trans_1n _ vred V₁ V₂).
-Notation jred_rtc J₁ J₂ := (clos_trans_1n _ jred J₁ J₂).
+Notation tred_tc M₁ M₂ := (clos_trans_1n _ tred M₁ M₂).
+Notation vred_tc V₁ V₂ := (clos_trans_1n _ vred V₁ V₂).
+Notation jred_tc J₁ J₂ := (clos_trans_1n _ jred J₁ J₂).
 
-Notation "M →+ₜ M'" := (tred_rtc M M') (at level 100).
-Notation "J →+ⱼ J'" := (jred_rtc J J') (at level 100).
-Notation "V →+ᵥ V'" := (vred_rtc V V') (at level 100).
+Notation "M →+ₜ M'" := (tred_tc M M') (at level 100).
+Notation "J →+ⱼ J'" := (jred_tc J J') (at level 100).
+Notation "V →+ᵥ V'" := (vred_tc V V') (at level 100).
+
+Notation tred_rtc M₁ M₂ := (clos_refl_trans _ tred M₁ M₂).
+Notation vred_rtc V₁ V₂ := (clos_refl_trans _ vred V₁ V₂).
+Notation jred_rtc J₁ J₂ := (clos_refl_trans _ jred J₁ J₂).
+
+Notation "M '→*ₜ' M'" := (tred_rtc M M') (at level 50).
+Notation "J '→*ⱼ' J'" := (jred_rtc J J') (at level 50).
+Notation "V '→*ᵥ' V'" := (vred_rtc V V') (at level 50).
+
+(* -------------------------------------------------------------------------- *)
+(* → and →* are preserved under fmap. *)
+
+Ltac cong H :=
+  induction H; [
+    constructor; constructor; assumption
+  | constructor 2
+  | econstructor 3; [
+      eassumption
+    | assumption ]
+  ].
+
+Lemma tred_value_cong {S : VSig} : ∀ (V V' : value S),
+  V →*ᵥ V' →
+  V →*ₜ V'.
+Proof.
+  intros V V' Hreds.
+  cong Hreds.
+Qed.
+
+Lemma tred_appl_cong {S : VSig} : ∀ (M M' N : term S),
+  M →*ₜ M' →
+  t_app M N →*ₜ t_app M' N.
+Proof.
+  intros M M' N Hreds.
+  cong Hreds.
+Qed.
+
+Lemma tred_appr_cong {S : VSig} : ∀ (M N N' : term S),
+  N →*ₜ N' →
+  t_app M N →*ₜ t_app M N'.
+Proof.
+  intros M M' N Hreds.
+  cong Hreds.
+Qed.
+
+Lemma tred_ctrl_cong {S : VSig} : ∀ (J J' : jump (incK S)),
+  J →*ⱼ J' →
+  t_ctrl J →*ₜ t_ctrl J'.
+Proof.
+  intros J J' Hreds.
+  cong Hreds.
+Qed.
+
+Lemma tred_plug {S : VSig} : ∀ (E : ectx S) (M M' : term S),
+  M →ₜ M' →
+  eplug E M →ₜ eplug E M'.
+Proof.
+  intros E M M' Hred.
+  induction E.
+  + term_simpl. apply Hred.
+  + term_simpl. constructor. apply IHE.
+  + term_simpl. constructor. apply IHE.
+Qed.
+
+Lemma tred_plug_cong {S : VSig} : ∀ (E : ectx S) (M M' : term S),
+  M →*ₜ M' →
+  eplug E M →*ₜ eplug E M'.
+Proof.
+  intros E M M' Hreds.
+  induction Hreds.
+  + constructor. term_simpl.
+    apply tred_plug. apply H.
+  + constructor 2.
+  + constructor 3 with (y := eplug E y).
+    apply IHHreds1.
+    apply IHHreds2.
+Qed.
+
+Lemma vred_lam_cong {S : VSig} : ∀ (M M' : term (incV S)),
+  M →*ₜ M' →
+  v_lam M →*ᵥ v_lam M'.
+Proof.
+  intros M M' Hreds.
+  cong Hreds.
+Qed.
+
+Lemma jred_jmp_cong {S : VSig} : ∀ (M M' : term S) q,
+  M →*ₜ M' →
+  j_jmp q M →*ⱼ j_jmp q M'.
+Proof.
+  intros M M' q Hreds.
+  cong Hreds.
+Qed.
+
+Lemma struct_subst_fmap {S T : VSig} (E : ectx S) (φ : prod_arr S T) :
+  struct_sub (shift (fmap φ E)) ∘ (φ ↑) ̂ ≡ (φ ↑) ̂ ∘ struct_sub (shift E).
+Proof.
+  constructor.
+  + intro x. term_simpl. reflexivity.
+  + intro k. destruct k.
+    - term_simpl.
+      rewrite <- map_to_bind.
+      term_simpl.
+      rewrite ecomp_pure.
+      reflexivity.
+    - term_simpl. reflexivity.
+Qed.
+
+Lemma tred_map {S T : VSig} : ∀ (M M' : term S) (φ : prod_arr S T),
+  M →ₜ M' →
+  fmap φ M →ₜ fmap φ M'
+with vred_map {S T : VSig} : ∀ (V V' : value S) (φ : prod_arr S T),
+  V →ᵥ V' →
+  fmap φ V →ᵥ fmap φ V'
+with jred_map {S T : VSig} : ∀ (J J' : jump S) (φ : prod_arr S T),
+  J →ⱼ J' →
+  fmap φ J →ⱼ fmap φ J'.
+Proof.
+(* tred_map *)
+{
+  intros M M' φ Hred.
+  induction Hred.
+  + term_simpl.
+    constructor.
+  + term_simpl.
+    unfold struct_subst.
+    erewrite <- bind_map_comm.
+    - apply tred_C_L.
+    - replace (e_appl e_hole (shift (fmap φ N))) with (shift (fmap φ (e_appl e_hole N))) by reflexivity.
+      replace (e_appl e_hole (shift N)) with (shift (e_appl e_hole N)) by reflexivity.
+      apply struct_subst_fmap.
+  + term_simpl.
+    unfold struct_subst.
+    erewrite <- bind_map_comm.
+    - apply tred_C_R.
+    - replace (e_appr (shift (fmap φ V)) e_hole) with (shift (fmap φ (e_appr V e_hole))) by reflexivity.
+      replace (e_appr (shift V) e_hole) with (shift (e_appr V e_hole)) by reflexivity.
+      apply struct_subst_fmap.
+  + term_simpl. constructor. apply vred_map. apply H.
+  + term_simpl. constructor. apply IHHred.
+  + term_simpl. constructor. apply IHHred.
+  + term_simpl. constructor. apply jred_map. apply H.
+}
+(* vred_map *)
+{
+  intros V V' φ Hred.
+  induction Hred.
+  + term_simpl. constructor. apply tred_map. apply H.
+}
+(* jred_map *)
+{
+  intros J J' φ Hred.
+  induction Hred.
+  + term_simpl. constructor.
+  + term_simpl. constructor. apply tred_map. apply H.
+}
+Qed.
+
+Lemma treds_map {S T : VSig} : ∀ (M M' : term S) (φ : prod_arr S T),
+  M →*ₜ M' →
+  fmap φ M →*ₜ fmap φ M'
+with vreds_map {S T : VSig} : ∀ (V V' : value S) (φ : prod_arr S T),
+  V →*ᵥ V' →
+  fmap φ V →*ᵥ fmap φ V'
+with jreds_map {S T : VSig} : ∀ (J J' : jump S) (φ : prod_arr S T),
+  J →*ⱼ J' →
+  fmap φ J →*ⱼ fmap φ J'.
+Proof.
+(* treds_map *)
+{
+  intros M M' φ Hreds.
+  induction Hreds.
+  + constructor. apply tred_map. apply H.
+  + constructor 2.
+  + econstructor 3.
+    - apply IHHreds1.
+    - apply IHHreds2.
+}
+(* vreds_map *)
+{
+  intros M M' φ Hreds.
+  induction Hreds.
+  + constructor. apply vred_map. apply H.
+  + constructor 2.
+  + econstructor 3.
+    - apply IHHreds1.
+    - apply IHHreds2.
+}
+(* jreds_map *)
+{
+  intros M M' φ Hreds.
+  induction Hreds.
+  + constructor. apply jred_map. apply H.
+  + constructor 2.
+  + econstructor 3.
+    - apply IHHreds1.
+    - apply IHHreds2.
+}
+Qed.
+
+(* -------------------------------------------------------------------------- *)
+Lemma treds_ctrl_plug {S : VSig} (J : jump (incK S)) E :
+  eplug E (t_ctrl J) →*ₜ t_ctrl (struct_subst J (shift E)).
+Proof.
+  induction E as [| E IHE M | V E IHE ].
+  + term_simpl. rewrite struct_subst_pure. constructor 2.
+  + term_simpl. econstructor 3.
+    { apply tred_appl_cong.
+      apply IHE. }
+    econstructor 3.
+    { constructor. constructor. }
+    rewrite struct_subst_comp with (E₂ := e_appl e_hole M).
+    term_simpl. constructor 2.
+  + term_simpl. econstructor 3.
+    { apply tred_appr_cong.
+      apply IHE. }
+    econstructor 3.
+    { constructor. constructor. }
+    rewrite struct_subst_comp with (E₂ := e_appr V e_hole).
+    term_simpl. constructor 2.
+Qed.
+
