Lang/Syntax.v
@@ -63,6 +63,25 @@ Fixpoint eplug {A : VSig} (E : ectx A) (t : term A) : term A :=
   | e_appr v E  => t_app v (eplug E t)
   end.
 
+(* Composition of evaluation contexts: (ecomp E1 E2)[M] = E1[E2[M]] *)
+Fixpoint ecomp {S : VSig} (E1 : ectx S) (E2 : ectx S) : ectx S :=
+  match E1 with
+  | e_hole      => E2
+  | e_appl E1 t => e_appl (ecomp E1 E2) t
+  | e_appr v E1 => e_appr v (ecomp E1 E2)
+  end.
+
+Lemma ecomp_assoc {S : VSig} (E₁ E₂ E₃ : ectx S) :
+  ecomp E₃ (ecomp E₂ E₁) = ecomp (ecomp E₃ E₂) E₁.
+Proof.
+  induction E₃.
+  + term_simpl. reflexivity.
+  + term_simpl. f_equal.
+    apply IHE₃.
+  + term_simpl. f_equal.
+    apply IHE₃.
+Qed.
+
 (* We use structural substitution with jumps.
    J[q E/k] means replace every occurence of k N with q E[N] in J. *)
 Inductive ssub (A : VSig) : Type :=
@@ -101,6 +120,88 @@ Instance FMap_term  : FunctorCore term  := @tmap.
 Instance FMap_value : FunctorCore value := @vmap.
 Instance FMap_jump  : FunctorCore jump  := @jmap.
 
+Local Open Scope bind_scope.
+
+Lemma tmap_id {A : VSig} (φ : prod_arr A A) M (EQ : φ ≡ ı) : tmap φ M = M
+with  vmap_id {A : VSig} (φ : prod_arr A A) V (EQ : φ ≡ ı) : vmap φ V = V
+with  jmap_id {A : VSig} (φ : prod_arr A A) J (EQ : φ ≡ ı) : jmap φ J = J.
+Proof.
+(* tmap_id *)
+{
+  induction M as [? V | ? M₁ IHM₁ M₂ | ? J ].
+  + term_simpl. f_equal. apply vmap_id. apply EQ.
+  + term_simpl. f_equal.
+    - apply IHM₁. apply EQ.
+    - apply IHM₂. apply EQ.
+  + term_simpl. f_equal.
+    apply jmap_id.
+    apply lift_id.
+    apply EQ.
+}
+(* vmap_id *)
+{
+  induction V as [x | M].
+  + term_simpl. f_equal. apply EQ.
+  + term_simpl. f_equal.
+    apply tmap_id.
+    apply lift_id.
+    apply EQ.
+}
+(* jmap_id *)
+{
+  induction J as [q M].
+  + term_simpl. f_equal.
+    - destruct q.
+      * term_simpl. f_equal. apply EQ.
+      * term_simpl. reflexivity.
+    - apply tmap_id. apply EQ.
+}
+Qed.
+
+Lemma tmap_map_comp {S T U : VSig} (φ₂ : prod_arr T U) (φ₁ : prod_arr S T) φ M (EQ : φ₂ ∘ φ₁ ≡ φ) :
+  tmap φ₂ (fmap φ₁ M) = fmap φ M
+with vmap_map_comp {S T U : VSig} (φ₂ : prod_arr T U) (φ₁ : prod_arr S T) φ V (EQ : φ₂ ∘ φ₁ ≡ φ) :
+  vmap φ₂ (fmap φ₁ V) = fmap φ V
+with jmap_map_comp {S T U : VSig} (φ₂ : prod_arr T U) (φ₁ : prod_arr S T) φ J (EQ : φ₂ ∘ φ₁ ≡ φ) :
+  jmap φ₂ (fmap φ₁ J) = fmap φ J.
+Proof.
+(* tmap_map_comp *)
+{
+  induction M as [? V | ? M₁ IHM₁ M₂ | ? J].
+  + term_simpl. f_equal. apply vmap_map_comp. apply EQ.
+  + term_simpl. f_equal.
+    - apply IHM₁. apply EQ.
+    - apply IHM₂. apply EQ.
+  + term_simpl. f_equal.
+    apply jmap_map_comp.
+    apply lift_comp.
+    apply EQ.
+}
+(* vmap_map_comp *)
+{
+  induction V as [x | M].
+  + term_simpl. f_equal. apply EQ.
+  + term_simpl. f_equal.
+    apply tmap_map_comp.
+    apply lift_comp.
+    apply EQ.
+}
+(* jmap_map_comp *)
+{
+  induction J as [q M].
+  + term_simpl. f_equal.
+    - destruct q as [k |].
+      * term_simpl. f_equal. apply EQ.
+      * term_simpl. reflexivity.
+    - apply tmap_map_comp.
+      apply EQ.
+}
+Qed.
+
+Instance Functor_term  : Functor term  := {| map_id := @tmap_id; map_map_comp := @tmap_map_comp |}.
+Instance Functor_value : Functor value := {| map_id := @vmap_id; map_map_comp := @vmap_map_comp |}.
+Instance Functor_jump  : Functor jump  := {| map_id := @jmap_id; map_map_comp := @jmap_map_comp |}.
+
 Fixpoint emap {A B : VSig} (φ : prod_arr A B) (E : ectx A) : ectx B :=
   match E with
   | e_hole     => e_hole
@@ -109,6 +210,31 @@ Fixpoint emap {A B : VSig} (φ : prod_arr A B) (E : ectx A) : ectx B :=
   end.
 
 Instance FMap_ectx : FunctorCore ectx := @emap.
+
+Lemma emap_id {A : VSig} (φ : prod_arr A A) E (EQ : φ ≡ ı) : emap φ E = E.
+Proof.
+  induction E; term_simpl; f_equal; try apply map_id; assumption.
+Qed.
+
+Lemma emap_map_comp {S T U : VSig} (φ₂ : prod_arr T U) (φ₁ : prod_arr S T) φ E (EQ : φ₂ ∘ φ₁ ≡ φ) :
+  emap φ₂ (fmap φ₁ E) = fmap φ E.
+Proof.
+  induction E; term_simpl; f_equal; try apply map_map_comp; assumption.
+Qed.
+
+Instance Functor_etcx : Functor ectx := {| map_id := @emap_id; map_map_comp := @emap_map_comp |}.
+
+Lemma emap_plug_comm {S T : VSig} (E : ectx S) (M : term S) (φ : prod_arr S T) :
+  fmap φ (eplug E M) = eplug (fmap φ E) (fmap φ M).
+Proof.
+  induction E; term_simpl; f_equal; assumption.
+Qed.
+
+Lemma ecomp_pure {S : VSig} (E : ectx S) :
+  ecomp E e_hole = E.
+Proof.
+  induction E; term_simpl; f_equal; assumption.
+Qed.
 
 Definition smap {A B : VSig} (φ : prod_arr A B) (s : ssub A) : ssub B :=
   match s with
@@ -176,15 +302,63 @@ Instance BindCore_term  : BindCore term  := @tbind.
 Instance BindCore_value : BindCore value := @vbind.
 Instance BindCore_jump  : BindCore jump  := @jbind.
 
-Definition struct_subst {A : VSig} (j : jump (incK A)) (E : ectx (incK A)) : jump (incK A) :=
-  bind {|
+Fixpoint ebind {A B : VSig} (φ : A {→} B) (E : ectx A) : ectx B :=
+  match E with
+  | e_hole     => e_hole
+  | e_appl E t => e_appl (ebind φ E) (tbind φ t)
+  | e_appr v E => e_appr (vbind φ v) (ebind φ E)
+  end.
+
+Instance BindCore_ectx : BindCore ectx := @ebind.
+
+Definition sbind {A B : VSig} (φ : A {→} B) (s : ssub A) : ssub B :=
+  match s with
+  | s_sub (k_var k) E =>
+    let (q, E') := sub_k φ k in s_sub q (ecomp E' (ebind φ E))
+  | s_sub k_tp E => s_sub k_tp (ebind φ E)
+  end.
+
+Instance BindCore_ssub : BindCore ssub := @sbind.
+
+Instance EqIndCore_VSub : EqIndCore VSub :=
+  {
+    equal := λ S T φ ψ,
+      (∀ x, sub_v φ x = sub_v ψ x)
+      ∧ (∀ k, sub_k φ k = sub_k ψ k)
+  }.
+
+Instance ArrowCore_VSub : ArrowCore VSub :=
+  {
+    arrow_id := λ S,
+      {|
+        sub_v := λ x, v_var x
+      ; sub_k := λ k, s_sub (k_var k) e_hole
+      |}
+  ; arrow_comp := λ A B C ψ φ,
+      {|
+        sub_v := λ (x : tv A), bind ψ (sub_v φ x)
+      ; sub_k := λ k,
+          let (q',  E2) := sub_k φ k in
+          match q' with
+          | k_tp     => s_sub k_tp (bind ψ E2)
+          | k_var k' =>
+            let (q'', E1) := sub_k ψ k' in
+            s_sub q'' (ecomp E1 (bind ψ E2))
+          end
+      |}
+  }.
+
+Definition struct_sub {A : VSig} E := {|
     sub_v := λ v, v_var v : value (incK A)
   ; sub_k := λ k,
       match k with
       | VZ   => s_sub (k_var VZ) E
       | VS y => s_sub (k_var (VS y)) e_hole
       end
-  |} j.
+  |}.
+
+Definition struct_subst {A : VSig} (j : jump (incK A)) (E : ectx (incK A)) : jump (incK A) :=
+  bind (struct_sub E) j.
 
 Instance SubstitutableCore_value : SubstitutableCore VSub value incV :=
   { mk_subst := λ A v,
@@ -209,3 +383,918 @@ Instance SubstitutableCore_jump : SubstitutableCore VSub ssub incK :=
     ; sub_v := λ (x : tv (incK A)), v_var x : value A
     |}
   }.
+
+Instance SubstCore_prod_arr_VSub : SubstCore prod_arr VSub :=
+  {
+    subst_of_arr := λ A B (φ : @prod_arr _ _ Arr Arr A B),
+      {|
+        sub_v := λ x, v_var (arr₁ φ x)
+      ; sub_k := λ k, s_sub (k_var (arr₂ φ k)) e_hole
+      |}
+  }.
+
+Program Instance EqInd_VSub : EqInd VSub.
+Next Obligation.
+  constructor.
+  + constructor.
+    - reflexivity.
+    - reflexivity.
+  + constructor.
+    rename x into φ₁, y into φ₂.
+    - intro x. symmetry. apply H.
+    - intro k. symmetry. apply H.
+  + constructor;
+    rename x into φ₁, y into φ₂, z into φ₃, H into Hφ₁φ₂, H0 into Hφ₂φ₃.
+    - intro x. etransitivity.
+      * apply Hφ₁φ₂.
+      * apply Hφ₂φ₃.
+    - intro k. etransitivity.
+      * apply Hφ₁φ₂.
+      * apply Hφ₂φ₃.
+Qed.
+
+Program Instance ASLiftInj_prod_arr_VSub_incK : ASLiftInj prod_arr VSub incK.
+Next Obligation.
+  constructor;
+  destruct EQ as [EQᵥ EQₖ].
+  + intro x.
+    specialize EQᵥ with x.
+    term_simpl in EQᵥ.
+
+    term_simpl. rewrite <- EQᵥ. term_simpl. reflexivity.
+  + intro k.
+    destruct k as [| k].
+    - term_simpl. reflexivity.
+    - term_simpl.
+      specialize EQₖ with k. term_simpl in EQₖ.
+      rewrite <- EQₖ.
+      term_simpl. reflexivity.
+Qed.
+
+Program Instance ASLiftInj_prod_arr_VSub_incV : ASLiftInj prod_arr VSub incV.
+Next Obligation.
+  constructor;
+  destruct EQ as [EQᵥ EQₖ].
+  + intro x.
+    destruct x as [| x].
+    - term_simpl. reflexivity.
+    - specialize EQᵥ with x.
+      term_simpl in EQᵥ.
+
+      term_simpl. rewrite <- EQᵥ. term_simpl. reflexivity.
+  + intro k.
+    specialize EQₖ with k. term_simpl in EQₖ.
+
+    term_simpl.
+    rewrite <- EQₖ.
+    term_simpl. reflexivity.
+Qed.
+
+Lemma tbind_map {S T : VSig} (φ : prod_arr S T) ψ (M : term S) (EQ : φ ̂ ≡ ψ) :
+  fmap φ M = bind ψ M
+ with vbind_map {S T : VSig} (φ : prod_arr S T) ψ (V : value S) (EQ : φ ̂ ≡ ψ) :
+  fmap φ V = bind ψ V
+ with jbind_map {S T : VSig} (φ : prod_arr S T) ψ (J : jump S) (EQ : φ ̂ ≡ ψ) :
+  fmap φ J = bind ψ J.
+Proof.
+(* tbind_map *)
+{
+  induction M.
+  + term_simpl. f_equal. apply vbind_map. apply EQ.
+  + term_simpl. f_equal.
+    - apply IHM1. apply EQ.
+    - apply IHM2. apply EQ.
+  + term_simpl. f_equal.
+    apply jbind_map.
+    apply lift_of.
+    apply EQ.
+}
+(* vbind_map *)
+{
+  induction V.
+  + term_simpl. apply EQ.
+  + term_simpl. f_equal.
+    apply tbind_map.
+    apply lift_of.
+    apply EQ.
+}
+(* jbind_map *)
+{
+  pose proof EQ as [_ EQₖ].
+
+  induction J.
+  + term_simpl.
+    destruct k.
+    - specialize EQₖ with k.
+      rewrite <- EQₖ.
+      term_simpl. f_equal.
+      apply tbind_map.
+      apply EQ.
+    - term_simpl. f_equal.
+      apply tbind_map.
+      apply EQ.
+}
+Qed.
+
+Instance BindMapPure_term  : BindMapPure term  := { bind_map := @tbind_map }.
+Instance BindMapPure_value : BindMapPure value := { bind_map := @vbind_map }.
+Instance BindMapPure_jump  : BindMapPure jump  := { bind_map := @jbind_map }.
+
+Lemma ebind_map {S T : VSig} (φ : prod_arr S T) ψ (E : ectx S) (EQ : φ ̂ ≡ ψ) :
+  fmap φ E = bind ψ E.
+Proof.
+  induction E.
+  + term_simpl. reflexivity.
+  + term_simpl. f_equal.
+    - apply IHE.
+    - apply tbind_map. apply EQ.
+  + term_simpl. f_equal.
+    - apply vbind_map. apply EQ.
+    - apply IHE.
+Qed.
+
+Instance BindMapPure_ectx : BindMapPure ectx := { bind_map := @ebind_map }.
+
+Lemma ecomp_fmap {S T : VSig} (E1 : ectx S) (E2 : ectx S) (φ : prod_arr S T) :
+  ecomp (fmap φ E1) (fmap φ E2) = fmap φ (ecomp E1 E2).
+Proof.
+  induction E1.
+  + term_simpl. reflexivity.
+  + term_simpl. f_equal.
+    apply IHE1.
+  + term_simpl. f_equal.
+    apply IHE1.
+Qed.
+
+Lemma ecomp_kshift {S : VSig} (E1 : ectx S) (E2 : ectx S) :
+  ecomp (shift E1) (shift E2) = shift (ecomp E1 E2).
+Proof.
+  apply ecomp_fmap.
+Qed.
+
+Lemma ecomp_vshift {S : VSig} (E1 : ectx S) (E2 : ectx S) :
+  ecomp (shift (Inc := incV) E1) (shift E2) = fmap mk_shift (ecomp E1 E2).
+Proof.
+  apply ecomp_fmap.
+Qed.
+
+Program Instance ASLiftComm_prod_arr_VSub_incK : ASLiftComm prod_arr VSub incK.
+Next Obligation.
+  term_simpl.
+  destruct EQ as [EQᵥ EQₖ]. simpl in EQₖ, EQᵥ.
+
+  constructor.
+  + intro x. term_simpl.
+    rewrite <- map_to_bind.
+    term_simpl. unfold shift. f_equal.
+
+    specialize EQᵥ with x. term_simpl in EQᵥ. rewrite <- map_to_bind in EQᵥ.
+
+    apply EQᵥ.
+  + intro k.
+    destruct k as [| k].
+    - term_simpl. reflexivity.
+    - term_simpl. specialize EQₖ with k.
+      destruct (sub_k g₂ (arr₂ f₂ k)) as [q₁ E₁].
+      destruct (sub_k g₁ k) as [q₂ E₂].
+      term_simpl.
+
+      apply (f_equal shift) in EQₖ.
+      term_simpl in EQₖ.
+      rewrite <- ecomp_kshift in EQₖ.
+      rewrite <- map_to_bind in EQₖ.
+      term_simpl in EQₖ.
+
+      rewrite <- map_to_bind.
+      rewrite fmap_liftA_shift_comm.
+
+      rewrite EQₖ.
+      destruct q₂; reflexivity.
+Qed.
+
+Program Instance ASLiftComm_prod_arr_VSub_incV : ASLiftComm prod_arr VSub incV.
+Next Obligation.
+  term_simpl.
+  destruct EQ as [EQᵥ EQₖ]. simpl in EQₖ, EQᵥ.
+
+  constructor.
+  + intro x. term_simpl.
+    destruct x as [| x].
+    - term_simpl. reflexivity.
+    - rewrite <- map_to_bind.
+      term_simpl. unfold shift. f_equal.
+
+      specialize EQᵥ with x. term_simpl in EQᵥ. rewrite <- map_to_bind in EQᵥ.
+
+      apply EQᵥ.
+  + intro k.
+    term_simpl. specialize EQₖ with k.
+    destruct (sub_k g₂ (arr₂ f₂ k)) as [q₁ E₁].
+    destruct (sub_k g₁ k) as [q₂ E₂].
+    term_simpl.
+
+    apply (f_equal (shift (Inc := incV))) in EQₖ.
+    term_simpl in EQₖ.
+    rewrite <- ecomp_vshift in EQₖ.
+    rewrite <- map_to_bind in EQₖ.
+    term_simpl in EQₖ.
+
+    rewrite <- map_to_bind.
+    rewrite fmap_liftA_shift_comm.
+
+    destruct q₂; apply EQₖ.
+Qed.
+
+Lemma tbind_map_comm {S T₁ T₂ U : VSig} (φ₁ : prod_arr T₁ U) (φ₂ : prod_arr S T₂) (ψ₁ : S {→} T₁) ψ₂ (M : term S) (EQ : ψ₂ ∘ φ₂ ̂ ≡ φ₁ ̂ ∘ ψ₁) :
+  bind ψ₂ (fmap φ₂ M) = fmap φ₁ (bind ψ₁ M)
+ with vbind_map_comm {S T₁ T₂ U : VSig} (φ₁ : prod_arr T₁ U) (φ₂ : prod_arr S T₂) (ψ₁ : S {→} T₁) ψ₂ (V : value S) (EQ : ψ₂ ∘ φ₂ ̂ ≡ φ₁ ̂ ∘ ψ₁) :
+  bind ψ₂ (fmap φ₂ V) = fmap φ₁ (bind ψ₁ V)
+ with jbind_map_comm {S T₁ T₂ U : VSig} (φ₁ : prod_arr T₁ U) (φ₂ : prod_arr S T₂) (ψ₁ : S {→} T₁) ψ₂ (J : jump S) (EQ : ψ₂ ∘ φ₂ ̂ ≡ φ₁ ̂ ∘ ψ₁) :
+  bind ψ₂ (fmap φ₂ J) = fmap φ₁ (bind ψ₁ J).
+Proof.
+(* tbind_map_comm *)
+{
+  induction M.
+  + term_simpl. f_equal. apply vbind_map_comm. apply EQ.
+  + term_simpl. f_equal.
+    - apply IHM1. apply EQ.
+    - apply IHM2. apply EQ.
+  + term_simpl. f_equal.
+    apply jbind_map_comm.
+    apply lift_comm.
+    apply EQ.
+}
+(* vbind_map_comm *)
+{
+  induction V.
+  + term_simpl.
+    destruct EQ as [EQ _]. specialize EQ with t.
+    term_simpl in EQ.
+    rewrite <- map_to_bind in EQ.
+    apply EQ.
+  + term_simpl. f_equal.
+    apply tbind_map_comm.
+    apply lift_comm.
+    apply EQ.
+}
+(* jbind_map_comm *)
+{
+  induction J as [q M].
+
+  + term_simpl.
+    destruct q as [k |].
+    - term_simpl.
+      pose proof EQ as [_ EQₖ]. specialize EQₖ with k.
+      term_simpl in EQₖ.
+
+      destruct (sub_k ψ₁ k) as [q E].
+      destruct (sub_k ψ₂ (arr₂ φ₂ k)) as [q' E'].
+
+      replace (BindCore_ectx T₁ U (φ₁ ̂) E) with (bind (φ₁ ̂) E) in EQₖ by reflexivity.
+      rewrite <- map_to_bind in EQₖ.
+      destruct q as [k' |].
+      * term_simpl. inversion EQₖ as [[Hq' HE']]. f_equal.
+        rewrite emap_plug_comm. f_equal.
+        ** rewrite ecomp_pure in HE'.
+           apply HE'.
+        ** apply tbind_map_comm.
+           apply EQ.
+      * term_simpl. inversion EQₖ as [[Hq' HE']]. f_equal.
+        rewrite emap_plug_comm. f_equal.
+        ** rewrite ecomp_pure in HE'.
+           apply HE'.
+        ** apply tbind_map_comm.
+           apply EQ.
+    - term_simpl. f_equal.
+      apply tbind_map_comm.
+      apply EQ.
+}
+Qed.
+
+Instance BindMapComm_term  : BindMapComm term  := { bind_map_comm := @tbind_map_comm }.
+Instance BindMapComm_value : BindMapComm value := { bind_map_comm := @vbind_map_comm }.
+Instance BindMapComm_jump  : BindMapComm jump  := { bind_map_comm := @jbind_map_comm }.
+
+Lemma ebind_map_comm {S T₁ T₂ U : VSig} (φ₁ : prod_arr T₁ U) (φ₂ : prod_arr S T₂) (ψ₁ : S {→} T₁) ψ₂ (E : ectx S) (EQ : ψ₂ ∘ φ₂ ̂ ≡ φ₁ ̂ ∘ ψ₁) :
+  bind ψ₂ (fmap φ₂ E) = fmap φ₁ (bind ψ₁ E).
+Proof.
+  induction E.
+  + term_simpl. reflexivity.
+  + term_simpl. f_equal.
+    - apply IHE.
+    - apply tbind_map_comm. apply EQ.
+  + term_simpl. f_equal.
+    - apply vbind_map_comm. apply EQ.
+    - apply IHE.
+Qed.
+
+Instance BindMapComm_ectx : BindMapComm ectx := { bind_map_comm := @ebind_map_comm }.
+
+Program Instance SubstFMap_prod_arr_VSub_value_incV : SubstFMap prod_arr VSub value incV.
+Next Obligation.
+  constructor.
+  + intro x. term_simpl.
+    destruct x.
+    - term_simpl.
+      rewrite <- map_to_bind.
+      reflexivity.
+    - term_simpl.
+      reflexivity.
+  + intro k. term_simpl. reflexivity.
+Qed.
+
+Program Instance SubstFMap_prod_arr_VSub_ssub_incK : SubstFMap prod_arr VSub ssub incK.
+Next Obligation.
+  constructor.
+  + intro x. term_simpl. reflexivity.
+  + intro k.
+    destruct k.
+    - term_simpl.
+      destruct v as [q E].
+      destruct q as [k |].
+      * term_simpl.
+        rewrite ecomp_pure.
+        rewrite <- map_to_bind.
+        reflexivity.
+      * term_simpl.
+        rewrite ecomp_pure.
+        rewrite <- map_to_bind.
+        reflexivity.
+    - term_simpl. reflexivity.
+Qed.
+
+Program Instance LiftSShift_prod_arr_VSub_incK : LiftSShift prod_arr VSub incK.
+Next Obligation.
+  constructor.
+  + intro x. term_simpl.
+    rewrite <- map_to_bind. reflexivity.
+  + intro k. term_simpl.
+    destruct (sub_k f k) as [q E].
+    term_simpl. destruct q as [k' |].
+    - term_simpl.
+      rewrite ecomp_pure.
+      rewrite <- map_to_bind.
+      reflexivity.
+    - term_simpl.
+      rewrite ecomp_pure.
+      rewrite <- map_to_bind.
+      reflexivity.
+Qed.
+
+Program Instance LiftSShift_prod_arr_VSub_incV : LiftSShift prod_arr VSub incV.
+Next Obligation.
+  constructor.
+  + intro x. term_simpl.
+    rewrite <- map_to_bind. reflexivity.
+  + intro k. term_simpl.
+    destruct (sub_k f k) as [q E].
+    term_simpl. destruct q as [k' |].
+    - term_simpl.
+      rewrite ecomp_pure.
+      rewrite <- map_to_bind.
+      reflexivity.
+    - term_simpl.
+      rewrite ecomp_pure.
+      rewrite <- map_to_bind.
+      reflexivity.
+Qed.
+
+Program Instance Liftable_VSub_incK : Liftable VSub incK.
+Next Obligation.
+  pose proof EQ as [EQᵥ EQₖ].
+  term_simpl in EQᵥ.
+  term_simpl in EQₖ.
+  constructor.
+  + intro x. term_simpl.
+    specialize EQᵥ with x. term_simpl in EQᵥ.
+    apply (f_equal shift) in EQᵥ. apply EQᵥ.
+  + intro k. destruct k as [| k].
+    - term_simpl. reflexivity.
+    - term_simpl. specialize EQₖ with k.
+      apply (f_equal shift) in EQₖ. apply EQₖ.
+Qed.
+Next Obligation.
+  pose proof EQ as [EQᵥ EQₖ]; term_simpl in EQᵥ; term_simpl in EQₖ;
+  term_simpl; term_simpl in EQ.
+  constructor.
+  + clear EQₖ. intro x. term_simpl.
+    specialize EQᵥ with x. term_simpl in EQᵥ.
+    f_equal. apply EQᵥ.
+  + clear EQᵥ. intro k. destruct k.
+    - term_simpl. reflexivity.
+    - term_simpl. specialize EQₖ with π.
+      destruct (sub_k g π) as [q E]. term_simpl.
+      destruct q as [k |].
+      * term_simpl. destruct (sub_k f k) as [q' E']. term_simpl.
+        rewrite ecomp_kshift.
+        replace (s_sub (shift q') (shift (ecomp E' (bind f E))))
+           with (shift (s_sub q' (ecomp E' (bind f E)))) by reflexivity.
+        f_equal.
+        apply EQₖ.
+      * term_simpl.
+        replace (s_sub k_tp (shift (bind f E)))
+           with (shift (s_sub k_tp (bind f E))) by reflexivity.
+        f_equal.
+        apply EQₖ.
+Qed.
+Next Obligation.
+  constructor.
+  rename x into φ, y into ψ.
+  + intro x. term_simpl. f_equal. apply H.
+  + intro k. destruct k.
+    - term_simpl. reflexivity.
+    - term_simpl. f_equal. apply H.
+Qed.
+
+Program Instance Liftable_VSub_incV : Liftable VSub incV.
+Next Obligation.
+  pose proof EQ as [EQᵥ EQₖ].
+  term_simpl in EQᵥ.
+  term_simpl in EQₖ.
+  constructor.
+  + intro x. destruct x as [| x].
+    - term_simpl. reflexivity.
+    - term_simpl. specialize EQᵥ with x. term_simpl in EQᵥ.
+      apply (f_equal (shift (Inc := incV))) in EQᵥ. apply EQᵥ.
+  + intro k. term_simpl.
+    term_simpl. specialize EQₖ with k.
+    apply (f_equal (shift (Inc := incV))) in EQₖ. apply EQₖ.
+Qed.
+Next Obligation.
+  pose proof EQ as [EQᵥ EQₖ]; term_simpl in EQᵥ; term_simpl in EQₖ;
+  term_simpl; term_simpl in EQ.
+  constructor.
+  + clear EQₖ. intro x. destruct x as [| x].
+    - term_simpl. reflexivity.
+    - term_simpl. specialize EQᵥ with x. term_simpl in EQᵥ.
+      f_equal. apply EQᵥ.
+  + clear EQᵥ. intro k. 
+    term_simpl. specialize EQₖ with k.
+    destruct (sub_k g k) as [q E]. term_simpl.
+    destruct q as [k' |].
+    * term_simpl. destruct (sub_k f k') as [q' E']. term_simpl.
+      rewrite ecomp_vshift.
+      apply (f_equal (shift (Inc := incV))) in EQₖ.
+      apply EQₖ.
+    * term_simpl.
+      apply (f_equal (shift (Inc := incV))) in EQₖ.
+      apply EQₖ.
+Qed.
+Next Obligation.
+  constructor.
+  rename x into φ, y into ψ.
+  + intro x. destruct x.
+    - term_simpl. reflexivity.
+    - term_simpl. f_equal. apply H.
+  + intro k. term_simpl. f_equal. apply H.
+Qed.
+
+Lemma tbind_pure {A : VSig} (φ : A {→} A) (M : term A) (EQ : φ ≡ ı) :
+  bind φ M = M
+ with vbind_pure {A : VSig} (φ : A {→} A) (V : value A) (EQ : φ ≡ ı) :
+  bind φ V = V
+ with jbind_pure {A : VSig} (φ : A {→} A) (J : jump A) (EQ : φ ≡ ı) :
+  bind φ J = J.
+Proof.
+(* tbind_pure *)
+{
+  induction M as [ S V | S M₁ IHM₁ M₂ IHM₂ |].
+  + term_simpl. f_equal. apply vbind_pure. apply EQ.
+  + term_simpl. f_equal.
+    - apply IHM₁. apply EQ.
+    - apply IHM₂. apply EQ.
+  + term_simpl. f_equal.
+    apply jbind_pure. apply lift_id. apply EQ.
+}
+(* vbind_pure *)
+{
+  induction V as [ x | M ].
+  + term_simpl. apply EQ.
+  + term_simpl. f_equal. apply tbind_pure. apply lift_id. apply EQ.
+}
+(* jbind_pure *)
+{
+  pose proof EQ as [_ EQₖ].
+  induction J as [q M].
+  + term_simpl. destruct q as [k |].
+    - specialize EQₖ with k.
+      destruct (sub_k φ k) as [q E]. term_simpl in EQₖ. inversion EQₖ as [[Hq HE]].
+      f_equal. term_simpl. apply tbind_pure. apply EQ.
+    - f_equal. apply tbind_pure. apply EQ.
+}
+Qed.
+
+Lemma eplug_fmap {A B : VSig} (φ : prod_arr A B) (E : ectx A) (M : term A) :
+  fmap φ (eplug E M) = eplug (fmap φ E) (fmap φ M).
+Proof.
+  induction E; term_simpl; f_equal; assumption.
+Qed.
+
+Lemma eplug_bind {A B : VSig} (φ : A {→} B) (E : ectx A) M :
+  eplug (bind φ E) (bind φ M) = bind φ (eplug E M).
+Proof.
+  induction E; term_simpl; f_equal; assumption.
+Qed.
+
+Lemma eplug_plug_comp {A : VSig} (E₂ E₁ : ectx A) (M : term A) :
+  eplug E₂ (eplug E₁ M) = eplug (ecomp E₂ E₁) M.
+Proof.
+  induction E₂; term_simpl; f_equal; assumption.
+Qed.
+
+Lemma tbind_bind_comp {A B C : VSig} (φ₂ : B {→} C) (φ₁ : A {→} B) ψ (M : term A) (EQ : φ₂ ∘ φ₁ ≡ ψ) :
+  bind φ₂ (bind φ₁ M) = bind ψ M
+ with vbind_bind_comp {A B C : VSig} (φ₂ : B {→} C) (φ₁ : A {→} B) ψ (V : value A) (EQ : φ₂ ∘ φ₁ ≡ ψ) :
+  bind φ₂ (bind φ₁ V) = bind ψ V
+ with jbind_bind_comp {A B C : VSig} (φ₂ : B {→} C) (φ₁ : A {→} B) ψ (J : jump A) (EQ : φ₂ ∘ φ₁ ≡ ψ) :
+  bind φ₂ (bind φ₁ J) = bind ψ J.
+Proof.
+(* tbind_bind_comp *)
+{
+  induction M as [ A V | A M₁ IHM₁ M₂ | A J].
+  + term_simpl. f_equal. apply vbind_bind_comp. apply EQ.
+  + term_simpl. f_equal.
+    - apply IHM₁. apply EQ.
+    - apply IHM₂. apply EQ.
+  + term_simpl. f_equal.
+    apply jbind_bind_comp. apply lift_comp. apply EQ.
+}
+(* vbind_bind_comp *)
+{
+  induction V as [ x | M ].
+  + term_simpl. apply EQ.
+  + term_simpl. f_equal. apply tbind_bind_comp. apply lift_comp. apply EQ.
+}
+(* jbind_bind_comp *)
+{
+  pose proof EQ as [_ EQₖ].
+
+  induction J as [q M].
+  term_simpl. destruct q as [k |].
+  + specialize EQₖ with k. inversion EQₖ as [Hsub].
+    destruct (sub_k φ₁ k) as [q E]. term_simpl.
+    destruct q as [k' |].
+    - destruct (sub_k φ₂ k') as [q' E'].
+      destruct (sub_k ψ k) as [q'' E''].
+      inversion Hsub. f_equal.
+      rewrite <- eplug_bind.
+      rewrite eplug_plug_comp. f_equal.
+      apply tbind_bind_comp. apply EQ.
+    - f_equal.
+      rewrite <- eplug_bind. f_equal.
+      apply tbind_bind_comp. apply EQ.
+  + term_simpl. f_equal.
+    apply tbind_bind_comp. apply EQ.
+}
+Qed.
+
+Instance Bind_term  : Bind term  := { bind_pure := @tbind_pure; bind_bind_comp := @tbind_bind_comp }.
+Instance Bind_value : Bind value := { bind_pure := @vbind_pure; bind_bind_comp := @vbind_bind_comp }.
+Instance Bind_jump  : Bind jump  := { bind_pure := @jbind_pure; bind_bind_comp := @jbind_bind_comp }.
+
+Lemma ebind_pure {A : VSig} (φ : A {→} A) (E : ectx A) (EQ : φ ≡ ı) :
+  bind φ E = E.
+Proof.
+  induction E as [| E IHE M | V E ].
+  + term_simpl. reflexivity.
+  + term_simpl. f_equal.
+    - apply IHE.
+    - apply tbind_pure. apply EQ.
+  + term_simpl. f_equal.
+    - apply vbind_pure. apply EQ.
+    - apply IHE.
+Qed.
+
+Lemma ebind_bind_comp {A B C : VSig} (φ₂ : B {→} C) (φ₁ : A {→} B) ψ (E : ectx A) (EQ : φ₂ ∘ φ₁ ≡ ψ) :
+  bind φ₂ (bind φ₁ E) = bind ψ E.
+Proof.
+  induction E as [| E IHE M | V E ].
+  + term_simpl. reflexivity.
+  + term_simpl. f_equal.
+    - apply IHE.
+    - apply tbind_bind_comp. apply EQ.
+  + term_simpl. f_equal.
+    - apply vbind_bind_comp. apply EQ.
+    - apply IHE.
+Qed.
+
+Instance Bind_ectx : Bind ectx := { bind_pure := @ebind_pure; bind_bind_comp := @ebind_bind_comp }.
+
+Program Instance SubstShift_prod_arr_VSub_value_incV : SubstShift prod_arr VSub value incV.
+Next Obligation.
+  constructor.
+  + intro x. term_simpl. reflexivity.
+  + intro k. term_simpl. reflexivity.
+Qed.
+
+Program Instance SubstShift_prod_arr_VSub_ssub_incK : SubstShift prod_arr VSub ssub incK.
+Next Obligation.
+  constructor.
+  + intro x. term_simpl. reflexivity.
+  + intro k. term_simpl. reflexivity.
+Qed.
+
+Program Instance Subst_prod_arr_VSub : Subst prod_arr VSub.
+Next Obligation.
+  constructor.
+  + intro x. term_simpl. reflexivity.
+  + intro k. term_simpl. reflexivity.
+Qed.
+Next Obligation.
+  constructor.
+  + intro x. term_simpl. reflexivity.
+  + intro k. term_simpl. reflexivity.
+Qed.
+Next Obligation.
+  constructor;
+  rename x into φ, y into ψ.
+  + intro x. term_simpl. f_equal. apply H.
+  + intro k. term_simpl. f_equal. f_equal. apply H.
+Qed.
+
+Definition VSub_id {A : VSig} :=
+  {| sub_v := λ x : tv A, v_var x
+   ; sub_k := λ k : kv A, s_sub (k_var k) e_hole |}.
+
+Lemma VSub_id_id {A : VSig} :
+  VSub_id ≡ arrow_id A.
+Proof.
+  constructor.
+  + intro x. reflexivity.
+  + intro k. reflexivity.
+Qed.
+
+Lemma VSub_comp {A B C : VSig} (f : B {→} C) g :
+  f ∘ g
+  ≡ {| sub_v := λ x : tv A, bind f (sub_v g x)
+     ; sub_k := λ k : kv A,
+        let (q', E2) := sub_k g k in
+        match q' with
+        | k_var k' =>
+          let (q'', E1) := sub_k f k' in
+          s_sub q'' (ecomp E1 (bind f E2))
+        | k_tp => s_sub k_tp (bind f E2)
+        end
+    |}.
+Proof.
+  constructor.
+  + intro x. term_simpl. reflexivity.
+  + intro k. term_simpl.
+    destruct (sub_k g k) as [q E].
+    destruct q as [k' |].
+    - destruct (sub_k f k') as [q' E']. term_simpl. reflexivity.
+    - term_simpl. reflexivity.
+Qed.
+
+Lemma ecomp_bind {S T : VSig} (E1 : ectx S) (E2 : ectx S) (φ : S {→} T) :
+  ecomp (bind φ E1) (bind φ E2) = bind φ (ecomp E1 E2).
+Proof.
+  induction E1.
+  + term_simpl. reflexivity.
+  + term_simpl. f_equal.
+    apply IHE1.
+  + term_simpl. f_equal.
+    apply IHE1.
+Qed.
+
+Lemma tbind_eq {A B : VSig} (φ ψ : A {→} B) (M : term A) :
+  φ ≡ ψ →
+  bind φ M = bind ψ M
+ with vbind_eq {A B : VSig} (φ ψ : A {→} B) (V : value A) :
+  φ ≡ ψ →
+  bind φ V = bind ψ V
+ with jbind_eq {A B : VSig} (φ ψ : A {→} B) (J : jump A) :
+  φ ≡ ψ →
+  bind φ J = bind ψ J.
+Proof.
+(* tbind_eq *)
+{
+  intro EQ.
+  induction M as [ A V | A M₁ IHM₁ M₂ | A J ].
+  + term_simpl. f_equal. apply vbind_eq. apply EQ.
+  + term_simpl. f_equal.
+    - apply IHM₁. apply EQ.
+    - apply IHM₂. apply EQ.
+  + term_simpl. f_equal. apply jbind_eq. apply lift_proper. apply EQ.
+}
+(* vbind_eq *)
+{
+  intro EQ.
+  induction V as [ x | M ].
+  + term_simpl. apply EQ.
+  + term_simpl. f_equal. apply tbind_eq. apply lift_proper. apply EQ.
+}
+(* jbind_eq *)
+{
+  intro EQ.
+  pose proof EQ as [EQᵥ EQₖ].
+
+  induction J as [q M].
+  + term_simpl.
+    destruct q as [k |].
+    - rewrite (EQₖ k).
+      destruct (sub_k ψ k) as [q E].
+      f_equal. f_equal. apply tbind_eq. apply EQ.
+    - f_equal. apply tbind_eq. apply EQ.
+}
+Qed.
+
+Lemma ebind_eq {A B : VSig} (φ ψ : A {→} B) (E : ectx A) :
+  φ ≡ ψ →
+  bind φ E = bind ψ E.
+Proof.
+  intro EQ.
+  induction E; term_simpl; f_equal;
+  try assumption; apply tbind_eq || apply vbind_eq; try assumption.
+Qed.
+
+Program Instance Arrow_VSub : Arrow VSub.
+Next Obligation.
+  constructor.
+  + intro x. term_simpl.
+    rewrite bind_pure.
+    - reflexivity.
+    - apply VSub_id_id.
+  + intro k. term_simpl.
+    destruct (sub_k f k) as [q E]. term_simpl.
+    destruct q; term_simpl; f_equal; apply bind_pure; apply VSub_id_id.
+Qed. Next Obligation.
+  constructor.
+  + intro x. term_simpl. reflexivity.
+  + intro k. term_simpl.
+    destruct (sub_k f k) as [q E].
+    rewrite ecomp_pure. reflexivity.
+Qed. Next Obligation.
+  constructor.
+  + intro x. term_simpl.
+    symmetry. apply bind_bind_comp.
+    apply VSub_comp.
+  + intro k. term_simpl.
+    destruct (sub_k h k) as [q₁ E₁]; term_simpl.
+    destruct q₁ as [k₁ |]; term_simpl.
+    - destruct (sub_k g k₁) as [q₂ E₂]; term_simpl.
+      destruct q₂ as [k₂ |]; term_simpl.
+      * destruct (sub_k f k₂) as [q₃ E₃]; term_simpl.
+        f_equal. rewrite <- ecomp_bind.
+        rewrite ecomp_assoc.
+        f_equal. symmetry. apply bind_bind_comp. apply VSub_comp.
+      * f_equal. rewrite <- ecomp_bind.
+        f_equal. symmetry. apply bind_bind_comp. apply VSub_comp.
+    - f_equal. symmetry. apply bind_bind_comp. apply VSub_comp.
+Qed. Next Obligation.
+  constructor;
+  pose proof H0 as [EQ₂ᵥ EQ₂ₖ];
+  pose proof H as [EQ₁ᵥ EQ₁ₖ];
+  rename x into φ₁, y into ψ₁, x0 into φ₂, y0 into ψ₂.
+  + intro x. term_simpl.
+    specialize EQ₂ᵥ with x. rewrite EQ₂ᵥ.
+    replace (sub_v ψ₂ x) with (bind ψ₂ (v_var x)) by reflexivity.
+    apply vbind_eq. apply H.
+  + intro k. term_simpl.
+    specialize EQ₂ₖ with k. rewrite EQ₂ₖ.
+    destruct (sub_k ψ₂ k) as [q E]; term_simpl.
+    destruct q as [k' |].
+    - specialize EQ₁ₖ with k'. rewrite EQ₁ₖ.
+      destruct (sub_k ψ₁ k') as [q' E'].
+      f_equal. f_equal.
+      apply ebind_eq. apply H.
+    - f_equal. apply ebind_eq. apply H.
+Qed.
+
+Program Instance SubstBind_VSub_value_incV : SubstBind VSub value incV.
+Next Obligation.
+  constructor.
+  + intro x. term_simpl.
+    destruct x as [| x].
+    - term_simpl. reflexivity.
+    - term_simpl. reflexivity.
+  + intro k. term_simpl.
+    destruct (sub_k f k) as [q E]. term_simpl.
+    destruct q as [k' |];
+      term_simpl; f_equal; apply ecomp_pure.
+Qed.
+
+Program Instance SubstBind_VSub_ssub_incK : SubstBind VSub ssub incK.
+Next Obligation.
+  constructor.
+  + intro x. term_simpl. reflexivity.
+  + intro k. term_simpl.
+    destruct k as [| k].
+    - destruct v as [q E].
+      destruct q as [k |].
+      * term_simpl. destruct (sub_k f k) as [q' E'].
+        rewrite ecomp_pure. reflexivity.
+      * term_simpl. rewrite ecomp_pure. reflexivity.
+    - term_simpl. destruct (sub_k f k) as [q E]. term_simpl.
+      destruct q as [k' |].
+      * term_simpl. rewrite ecomp_pure. reflexivity.
+      * term_simpl. rewrite ecomp_pure. reflexivity.
+Qed.
+
+Lemma struct_subst_pure {A : VSig} (J : jump (incK A)) :
+  struct_subst J e_hole = J.
+Proof.
+  unfold struct_subst.
+  apply bind_pure.
+  constructor.
+  + intro x. term_simpl. reflexivity.
+  + intro k. destruct k as [| k].
+    - term_simpl. reflexivity.
+    - term_simpl. reflexivity.
+Qed.
+
+Lemma fmap_struct_sub_comm {A B : VSig} (φ : prod_arr A B) E :
+   (φ ↑) ̂ ∘ struct_sub (shift E) ≡ struct_sub (fmap (φ ↑) (shift E)) ∘ (φ ↑) ̂.
+Proof.
+  constructor.
+  + intro x. term_simpl. reflexivity.
+  + intro k. term_simpl.
+    destruct k as [| k].
+    - term_simpl.
+      rewrite ecomp_pure.
+      rewrite <- map_to_bind. f_equal.
+      unfold shift.
+      rewrite !map_map_comp'; reflexivity.
+    - term_simpl. reflexivity.
+Qed.
+
+Lemma bind_struct_sub_comm {A B : VSig} (φ : A {→} B) (E : ectx A) :
+  φ ↑ ∘ struct_sub (shift E) ≡ struct_sub (bind (φ ↑) (shift E)) ∘ φ ↑.
+Proof.
+  constructor.
+  + intro x. term_simpl.
+
+    destruct (sub_v φ x).
+    - term_simpl. reflexivity.
+    - term_simpl. f_equal.
+      rewrite map_to_bind.
+      rewrite bind_bind_comp'.
+      rewrite lift_of_arrow.
+      rewrite lift_comp by reflexivity.
+      apply bind_proper; reflexivity.
+  + intro k. destruct k as [| k].
+    - term_simpl. rewrite ecomp_pure. reflexivity.
+    - term_simpl. destruct (sub_k φ k) as [q E']. term_simpl.
+      destruct q as [k' |].
+      * term_simpl. rewrite ecomp_pure. f_equal.
+        unfold shift.
+        rewrite map_to_bind.
+        rewrite bind_bind_comp'.
+        apply bind_proper; reflexivity.
+      * term_simpl. rewrite ecomp_pure. f_equal.
+        unfold shift.
+        rewrite map_to_bind.
+        rewrite bind_bind_comp'.
+        apply bind_proper; reflexivity.
+Qed.
+
+Lemma bind_struct_subst {A B : VSig} (φ : A {→} B) (J : jump (incK A)) (E : ectx A) :
+  bind (φ ↑) (struct_subst J (shift E)) = struct_subst (bind (φ ↑) J) (bind (φ ↑) (shift E)).
+Proof.
+  unfold struct_subst.
+  rewrite !bind_bind_comp'.
+  apply bind_proper; [| reflexivity].
+  apply bind_struct_sub_comm.
+Qed.
+
+Lemma fmap_struct_subst {A B : VSig} (φ : prod_arr A B) (J : jump (incK A)) (E : ectx A) :
+  fmap (φ ↑) (struct_subst J (shift E)) = struct_subst (fmap (φ ↑) J) (fmap (φ ↑) (shift E)).
+Proof.
+  unfold struct_subst. symmetry.
+  erewrite bind_map_comm.
+  + reflexivity.
+  + symmetry. apply fmap_struct_sub_comm.
+Qed.
+
+Lemma struct_subst_comp {A : VSig} (E₂ E₁ : ectx A) (J : jump (incK A)) :
+  struct_subst (struct_subst J (shift E₁)) (shift E₂) = struct_subst J (shift (ecomp E₂ E₁)).
+Proof.
+  unfold struct_subst.
+  rewrite !bind_bind_comp'.
+  apply bind_proper; [| reflexivity ].
+
+  constructor.
+  + intro x. term_simpl. reflexivity.
+  + intro k. destruct k as [| k].
+    - term_simpl. f_equal.
+      rewrite <- ecomp_kshift. f_equal.
+      unfold shift.
+      rewrite !map_to_bind with (f := mk_shift).
+      rewrite bind_bind_comp'.
+      apply bind_proper; reflexivity.
+    - term_simpl. f_equal.
+Qed.
+
+Lemma subst_struct_subst {A : VSig} (E₂ E₁ : ectx A) q J :
+  subst (struct_subst J (shift E₁)) (s_sub q E₂) = subst J (s_sub q (ecomp E₂ E₁)).
+Proof.
+  unfold subst, struct_subst.
+  rewrite !bind_bind_comp'.
+  apply bind_proper; [| reflexivity ].
+
+  constructor.
+  + intro x. term_simpl. reflexivity.
+  + intro k. destruct k as [| k].
+    - term_simpl. f_equal.
+    - term_simpl. f_equal.
+Qed.
