Lang/Confluence.v
@@ -1,0 +1,1882 @@
+Require Import Utf8.
+Require Import Binding.Lib Binding.Product Binding.Set.
+Require Import Syntax Semantics.
+Require Import Relation_Operators.
+
+(* Formalization based on:
+    [1] Baba Kensuke, Sachio Hirokawa, Ken-Etsu Fujita:
+        Parallel Reduction in Type Free λμ-Calculus. Electronic Notes in Theoretical Computer Science. 2001;42:52–66.
+    [2] Herman Geuvers, Robbert Krebbers, James McKinna:
+        The λμᵀ-calculus. Annals of Pure and Applied Logic. 2012;164(6):676-701.
+    [3] Programming Language Foundations in Agda - Confluence:
+        https://plfa.inf.ed.ac.uk/Confluence/
+*)
+
+Reserved Notation "M '⇉ₜ' M'" (at level 67).
+Reserved Notation "V '⇉ᵥ' V'" (at level 67).
+Reserved Notation "J '⇉ⱼ' J'" (at level 67).
+Reserved Notation "E '⇉ₑ' E'" (at level 67).
+
+(* We prove confluence in the typical way by defining a parallel reduction relation ⇉.
+  It corresponds to reducing many redexes in a term simultaneously. We then show that:
+    - ⇉ is confluent (by defining a complete development),
+    - ⇉ ⊆ →* ⊆ ⇉*,
+  which implies that the original reduction is confluent.
+
+  It's worth to note that the naive definition of ⇉ doesn't work [1].
+  To fix this, a slight change is needed for the rule jpar_C_idem. *)
+Inductive tpar {S : VSig} : term S → term S → Prop :=
+  | tpar_beta : ∀ M M' (V V' : value S),
+    M ⇉ₜ M' →
+    V ⇉ᵥ V' →
+    t_app (v_lam M) V ⇉ₜ subst M' V'
+  | tpar_C_L : ∀ J J' N N',
+    J ⇉ⱼ J' →
+    N ⇉ₜ N' →
+    t_app (t_ctrl J) N ⇉ₜ t_ctrl (struct_subst J' (e_appl e_hole (shift N')))
+  | tpar_C_R : ∀ J J' (V V' : value S),
+    J ⇉ⱼ J' →
+    V ⇉ᵥ V' →
+    t_app V (t_ctrl J) ⇉ₜ t_ctrl (struct_subst J' (e_appr (shift V') e_hole))
+
+  | tpar_value : ∀ V V',
+    V ⇉ᵥ V' →
+    V ⇉ₜ V'
+  | tpar_app : ∀ M M' N N',
+    M ⇉ₜ M' →
+    N ⇉ₜ N' →
+    t_app M N ⇉ₜ t_app M' N'
+  | tpar_ctrl : ∀ J J',
+    J ⇉ⱼ J' →
+    t_ctrl J ⇉ₜ t_ctrl J'
+with vpar {S : VSig} : value S → value S → Prop :=
+  | vpar_var : ∀ x,
+    v_var x ⇉ᵥ v_var x
+  | vpar_lam : ∀ M M',
+    M ⇉ₜ M' →
+    v_lam M ⇉ᵥ v_lam M'
+with jpar {S : VSig} : jump S → jump S → Prop :=
+  (* The naive definition would be:
+        j_jmp q (t_ctrl J) ⇉ⱼ subst J' (s_sub q e_hole).
+     However, this doesn't work. We need to generalize it for any evaluation context. *)
+  | jpar_C_idem : ∀ (q : katom S) E E' J J',
+    J ⇉ⱼ J' →
+    E ⇉ₑ E' →
+    j_jmp q (eplug E (t_ctrl J)) ⇉ⱼ subst J' (s_sub q E')
+
+  | jpar_jmp : ∀ q M M',
+    M ⇉ₜ M' →
+    j_jmp q M ⇉ⱼ j_jmp q M'
+with epar {S : VSig} : ectx S → ectx S → Prop :=
+  | epar_hole :
+    e_hole ⇉ₑ e_hole
+  | epar_appl : ∀ E E' M M',
+    E ⇉ₑ E' →
+    M ⇉ₜ M' →
+    e_appl E M ⇉ₑ e_appl E' M'
+  | epar_appr : ∀ V V' E E',
+    V ⇉ᵥ V' →
+    E ⇉ₑ E' →
+    e_appr V E ⇉ₑ e_appr V' E'
+
+where "M ⇉ₜ M'" := (tpar M M')
+  and "V ⇉ᵥ V'" := (vpar V V')
+  and "J ⇉ⱼ J'" := (jpar J J')
+  and "E ⇉ₑ E'" := (epar E E').
+
+Notation tpar_rtc M₁ M₂ := (clos_refl_trans _ tpar M₁ M₂).
+Notation vpar_rtc V₁ V₂ := (clos_refl_trans _ vpar V₁ V₂).
+Notation jpar_rtc J₁ J₂ := (clos_refl_trans _ jpar J₁ J₂).
+
+Notation "M '⇉*ₜ' M'" := (tpar_rtc M M') (at level 50).
+Notation "J '⇉*ⱼ' J'" := (jpar_rtc J J') (at level 50).
+Notation "V '⇉*ᵥ' V'" := (vpar_rtc V V') (at level 50).
+
+Lemma tpar_eplug {S : VSig} (E E' : ectx S) (M M' : term S) :
+  E ⇉ₑ E' →
+  M ⇉ₜ M' →
+  eplug E M ⇉ₜ eplug E' M'.
+Proof.
+  intros HparE HparM.
+  induction HparE;
+    repeat (term_simpl; constructor || auto).
+Qed.
+
+Lemma tpar_lam_invert {S : VSig} (M M' : term (incV S)) :
+  v_lam M ⇉ₜ v_lam M' →
+  M ⇉ₜ M'.
+Proof.
+  intro Hpar.
+  inversion Hpar; subst.
+  inversion H1; subst.
+  apply H2.
+Qed.
+
+Lemma tpar_value_invert {S : VSig} (V V' : value S) :
+  V ⇉ₜ V' →
+  V ⇉ᵥ V'.
+Proof.
+  intro Hpar. inversion Hpar; assumption.
+Qed.
+
+Lemma tpar_ctrl_invert {S : VSig} (J J' : jump (incK S)) :
+  t_ctrl J ⇉ₜ t_ctrl J' →
+  J ⇉ⱼ J'.
+Proof.
+  intro Hpar. inversion Hpar; assumption.
+Qed.
+
+(* -------------------------------------------------------------------------- *)
+(* ⇉ is reflexive. *)
+
+Lemma tpar_refl {S : VSig} : ∀ (M : term S),
+  M ⇉ₜ M
+with vpar_refl {S : VSig} : ∀ (V : value S),
+  V ⇉ᵥ V
+with jpar_refl {S : VSig} : ∀ (J : jump S),
+  J ⇉ⱼ J.
+Proof.
+(* tpar_refl *)
+{
+  induction M.
+  + constructor. apply vpar_refl.
+  + constructor.
+    - apply IHM1.
+    - apply IHM2.
+  + constructor. apply jpar_refl.
+}
+(* vpar_refl *)
+{
+  induction V.
+  + constructor.
+  + constructor. apply tpar_refl.
+}
+(* jpar_refl *)
+{
+  induction J.
+  constructor. apply tpar_refl.
+}
+Qed.
+
+Lemma epar_refl {S : VSig} : ∀ (E : ectx S),
+  E ⇉ₑ E.
+Proof.
+  intro E.
+  induction E; constructor; assumption || apply tpar_refl || apply vpar_refl.
+Qed.
+
+(* -------------------------------------------------------------------------- *)
+(* → ⊆ ⇉ and →* ⊆ ⇉*. *)
+
+Lemma tred_par {S : VSig} : ∀ (M N : term S),
+  M →ₜ N →
+  M ⇉ₜ N
+with vred_par {S : VSig} : ∀ (V V' : value S),
+  V →ᵥ V' →
+  V ⇉ᵥ V'
+with jred_par {S : VSig} : ∀ (J J' : jump S),
+  J →ⱼ J' →
+  J ⇉ⱼ J'.
+Proof.
+(* tred_par *)
+{
+  intros M N Hred.
+  induction Hred.
+  + constructor 1 with (V' := V).
+    - apply tpar_refl.
+    - apply vpar_refl.
+  + constructor.
+    - apply jpar_refl.
+    - apply tpar_refl.
+  + econstructor.
+    - apply jpar_refl.
+    - apply vpar_refl.
+  + constructor.
+    apply vred_par. apply H.
+  + constructor.
+    - apply IHHred.
+    - apply tpar_refl.
+  + constructor.
+    - apply tpar_refl.
+    - apply IHHred.
+  + constructor.
+    apply jred_par. apply H.
+}
+(* vred_par *)
+{
+  intros V V' Hred.
+  induction Hred.
+  constructor.
+  apply tred_par. apply H.
+}
+(* jred_par *)
+{
+  intros J J' Hred.
+  induction Hred.
+  + econstructor 1 with (E := e_hole).
+    - apply jpar_refl.
+    - apply epar_refl.
+  + constructor.
+    apply tred_par. apply H.
+}
+Qed.
+
+Lemma treds_pars {S : VSig} : ∀ (M N : term S),
+  M →*ₜ N →
+  M ⇉*ₜ N
+with vreds_pars {S : VSig} : ∀ (V V' : value S),
+  V →*ᵥ V' →
+  V ⇉*ᵥ V'
+with jreds_pars {S : VSig} : ∀ (J J' : jump S),
+  J →*ⱼ J' →
+  J ⇉*ⱼ J'.
+Proof.
+(* treds_pars *)
+{
+  intros M N Hreds.
+  induction Hreds.
+  + constructor. apply tred_par. apply H.
+  + constructor 2.
+  + econstructor 3.
+    - apply IHHreds1.
+    - apply IHHreds2.
+}
+(* vreds_pars *)
+{
+  intros V V' Hreds.
+  induction Hreds.
+  + constructor. apply vred_par. apply H.
+  + constructor 2.
+  + econstructor 3.
+    - apply IHHreds1.
+    - apply IHHreds2.
+}
+(* jreds_pars *)
+{
+  intros J J' Hreds.
+  induction Hreds.
+  + constructor. apply jred_par. apply H.
+  + constructor 2.
+  + econstructor 3.
+    - apply IHHreds1.
+    - apply IHHreds2.
+}
+Qed.
+
+(* -------------------------------------------------------------------------- *)
+(* ⇉ ⊆ →* and ⇉* ⊆ →*. *)
+
+Lemma tpar_reds {S : VSig} (M N : term S) :
+  M ⇉ₜ N →
+  M →*ₜ N
+with vpar_reds {S : VSig} (V V' : value S) :
+  V ⇉ᵥ V' →
+  V →*ᵥ V'
+with jpar_reds {S : VSig} (J J' : jump S) :
+  J ⇉ⱼ J' →
+  J →*ⱼ J'
+with epar_reds {S : VSig} (E E' : ectx S) M :
+  E ⇉ₑ E' →
+  eplug E M →*ₜ eplug E' M.
+Proof.
+(* tpar_reds *)
+{
+  intro Hpar.
+  induction Hpar.
+  + constructor 3 with (y := t_app (v_lam M') V).
+    { apply tred_appl_cong.
+      apply tred_value_cong.
+      apply vred_lam_cong.
+      apply IHHpar. }
+    constructor 3 with (y := t_app (v_lam M') V').
+    { apply tred_appr_cong.
+      apply tred_value_cong.
+      apply vpar_reds.
+      apply H. }
+    constructor. constructor.
+  + constructor 3 with (y := t_app (t_ctrl J') N).
+    { apply tred_appl_cong.
+      apply tred_ctrl_cong.
+      apply jpar_reds.
+      apply H. }
+    constructor 3 with (y := t_app (t_ctrl J') N').
+    { apply tred_appr_cong.
+      apply IHHpar. }
+    constructor. constructor.
+  + constructor 3 with (y := t_app V' (t_ctrl J)).
+    { apply tred_appl_cong.
+      apply tred_value_cong.
+      apply vpar_reds.
+      apply H0. }
+    constructor 3 with (y := t_app V' (t_ctrl J')).
+    { apply tred_appr_cong.
+      apply tred_ctrl_cong.
+      apply jpar_reds.
+      apply H. }
+    constructor. constructor.
+  + apply tred_value_cong.
+    apply vpar_reds.
+    apply H.
+  + constructor 3 with (y := t_app M' N).
+    - apply tred_appl_cong.
+      apply IHHpar1.
+    - apply tred_appr_cong.
+      apply IHHpar2.
+  + apply tred_ctrl_cong.
+    apply jpar_reds.
+    apply H.
+}
+(* vpar_reds *)
+{
+  intro Hpar.
+  induction Hpar.
+  + constructor 2.
+  + apply vred_lam_cong.
+    apply tpar_reds.
+    apply H.
+}
+(* jpar_reds *)
+{
+  intro Hpar.
+  induction Hpar.
+  + constructor 3 with (y := j_jmp q (eplug E (t_ctrl J'))).
+    { apply jred_jmp_cong.
+      apply tred_plug_cong.
+      apply tred_ctrl_cong.
+      apply IHHpar. }
+    econstructor 3.
+    { apply jred_jmp_cong.
+      apply epar_reds.
+      apply H. }
+    econstructor 3.
+    { apply jred_jmp_cong.
+      apply treds_ctrl_plug. }
+    econstructor 3.
+    { constructor. constructor. }
+    rewrite subst_struct_subst.
+    term_simpl. constructor 2.
+  + apply jred_jmp_cong.
+    apply tpar_reds.
+    apply H.
+}
+(* epar_reds *)
+{
+  intro Hpar.
+  induction Hpar.
+  + term_simpl. constructor 2.
+  + term_simpl.
+    econstructor 3.
+    { apply tred_appl_cong.
+      apply IHHpar. }
+    econstructor 3.
+    { apply tred_appr_cong.
+      apply tpar_reds.
+      apply H. }
+    constructor 2.
+  + term_simpl.
+    econstructor 3.
+    { apply tred_appr_cong.
+      apply IHHpar. }
+    econstructor 3.
+    { apply tred_appl_cong.
+      apply tred_value_cong.
+      apply vpar_reds.
+      apply H. }
+    econstructor 2.
+}
+Qed.
+
+Lemma tpars_reds {S : VSig} (M N : term S) :
+  M ⇉*ₜ N →
+  M →*ₜ N
+with vpars_reds {S : VSig} (V V' : value S) :
+  V ⇉*ᵥ V' →
+  V →*ᵥ V'
+with jpars_reds {S : VSig} (J J' : jump S) :
+  J ⇉*ⱼ J' →
+  J →*ⱼ J'.
+Proof.
+all: (
+  intros Hpar;
+  induction Hpar; [
+    apply tpar_reds || apply vpar_reds || apply jpar_reds; apply H
+  | constructor 2
+  | econstructor 3; [
+      apply IHHpar1
+    | apply IHHpar2 ]]).
+Qed.
+
+(* -------------------------------------------------------------------------- *)
+(* complete development *)
+
+(* The complete development is obtained by contracting all redexes of a term. *)
+Fixpoint tcd {S : VSig} (M : term S) { struct M } : term S :=
+  match M with
+  | t_value V => t_value (vcd V)
+  | t_app (v_lam M₁) (t_value V₂) => subst (tcd M₁) (vcd V₂)
+  | t_app (t_ctrl J) M₂ => t_ctrl (struct_subst (jcd J) (e_appl e_hole (shift (tcd M₂))))
+  | t_app (t_value V₁) (t_ctrl J) => t_ctrl (struct_subst (jcd J) (e_appr (shift (vcd V₁)) e_hole))
+  | t_app M₁ M₂ => t_app (tcd M₁) (tcd M₂)
+  | t_ctrl J => t_ctrl (jcd J)
+  end
+with vcd {S : VSig} (V : value S) { struct V } : value S :=
+  match V with
+  | v_var x => v_var x
+  | v_lam M => v_lam (tcd M)
+  end
+with jcd {S : VSig} (J : jump S) { struct J } : jump S :=
+  match J with
+  | j_jmp q M =>
+    match unplug_ctrl M with
+    | Some (E, J) => subst J (s_sub q E)
+    | None => j_jmp q (tcd M)
+    end
+  end
+(* return Some (ecd E, jcd J) iff M = eplug E (t_ctrl J) *)
+with unplug_ctrl {S : VSig} (M : term S) : option (ectx S * jump (incK S)) :=
+  match M with
+  | t_value V => None
+  | t_app (t_value V₁) M₂ =>
+    match unplug_ctrl M₂ with
+    | Some (E, J) => Some (e_appr (vcd V₁) E, J)
+    | None => None
+    end
+  | t_app M₁ M₂ =>
+    match unplug_ctrl M₁ with
+    | Some (E, J) => Some (e_appl E (tcd M₂), J)
+    | None => None
+    end
+  | t_ctrl J => Some (e_hole, jcd J)
+  end.
+
+Fixpoint ecd {S : VSig} (E : ectx S) : ectx S :=
+  match E with
+  | e_hole => e_hole
+  | e_appl E M => e_appl (ecd E) (tcd M)
+  | e_appr V E => e_appr (vcd V) (ecd E)
+  end.
+
+Lemma unplug_ctrl_correct1 {S : VSig} (M : term S) :
+  ∀ E J, unplug_ctrl M = Some (E, J)
+  → (∀ E' J', M = eplug E' (t_ctrl J') → ecd E' = E ∧ jcd J' = J).
+Proof.
+  intros E J Hunplug F K HM.
+  induction M as [ S V | S M₁ IHM₁ M₂ | S J' ].
+  + discriminate Hunplug.
+  + destruct M₁ as [ V₁ | N₁ N₂ | J₂ ].
+    - term_simpl in Hunplug.
+      destruct (unplug_ctrl M₂) as [[E' J'] |]; [| discriminate ].
+      inversion Hunplug as [[HE' HJ']]; clear HE'.
+      rewrite HJ' in *; clear HJ'.
+      destruct F; try discriminate.
+      * destruct F; try discriminate.
+      * term_simpl in HM.
+        specialize IHM₂ with E' J F K.
+        inversion HM as [[HV₁ HM₂]].
+        destruct (IHM₂ (eq_refl (Some (E', J))) HM₂) as [HF HK].
+        split; [| apply HK ].
+        term_simpl. f_equal. apply HF.
+    - term_simpl in Hunplug.
+      destruct N₁ as [ V₁ | U₁ U₂ | J₁ ].
+      * destruct (unplug_ctrl N₂) as [[E' J'] |] eqn:HunN₂; [| discriminate ].
+        inversion Hunplug as [[HE' HJ']]; clear HE'.
+        rewrite HJ' in *; clear HJ'.
+        destruct F; try discriminate.
+        term_simpl in HM.
+        inversion HM as [[HV₁ HM₂]].
+        specialize IHM₁ with (e_appr (vcd V₁) E') J F K.
+        apply IHM₁ in HV₁ as [HF HK].
+        { split; [| apply HK ]. term_simpl.
+          f_equal. apply HF. }
+        { term_simpl. rewrite HunN₂. reflexivity. }
+      * destruct (unplug_ctrl (t_app U₁ U₂)) as [[E' J'] |] eqn:Hunapp; [| discriminate ].
+        inversion Hunplug as [[HE' HJ']]; clear HE'.
+        rewrite HJ' in *; clear HJ'.
+        destruct F; try discriminate.
+        term_simpl in HM.
+        inversion HM as [[Happ HM₂]].
+        specialize IHM₁ with (e_appl E' (tcd N₂)) J F K.
+        apply IHM₁ in Happ as [HF HK].
+        { split; [| apply HK ]. term_simpl.
+          f_equal. apply HF. }
+
+        remember (t_app U₁ U₂) as N₁.
+        term_simpl. destruct N₁; try discriminate; rewrite HeqN₁ in *.
+        rewrite Hunapp. reflexivity.
+      * term_simpl in Hunplug.
+        inversion Hunplug as [[HE HJ]]; clear HE.
+        rewrite HJ in *.
+        destruct F; try discriminate.
+        inversion HM as [[Happ HM₂]].
+        specialize IHM₁ with (e_appl e_hole (tcd N₂)) J F K.
+        apply IHM₁ in Happ as [HF HK].
+        { split; [| apply HK ]. term_simpl.
+          f_equal. apply HF. }
+
+        term_simpl. rewrite HJ. reflexivity.
+    - term_simpl in Hunplug.
+      inversion Hunplug as [[HE HJ]]; clear HE.
+      destruct F; try discriminate.
+      inversion HM as [[Hctrl HM₂]].
+      specialize IHM₁ with e_hole (jcd J₂) F K.
+      apply IHM₁ in Hctrl as [HF HK].
+      { split; [| apply HK ]. term_simpl.
+        f_equal. apply HF. }
+
+      term_simpl. reflexivity.
+  + term_simpl in Hunplug.
+    inversion Hunplug as [[HE HJ]].
+    destruct F; try discriminate.
+    inversion HM.
+    auto.
+Qed.
+
+Lemma unplug_ctrl_correct2 {S : VSig} (M : term S) E' J' E J :
+  M = eplug E' (t_ctrl J') →
+  ecd E' = E →
+  jcd J' = J →
+  unplug_ctrl M = Some (E, J).
+Proof.
+  intros HM HE HJ.
+  induction M as [ S V | S M₁ IHM₁ M₂ | S K ].
+  + destruct E'; discriminate.
+  + destruct M₁ as [ V₁ | N₁ N₂ | J₂ ].
+    - destruct E'; try discriminate.
+      { term_simpl in HM. destruct E'; try discriminate. }
+      term_simpl in HE.
+      destruct E as [| | v' E ]; try discriminate.
+      inversion HE as [[Hvcd Hecd]].
+      inversion HM as [[HV₁ HM₂]]. rewrite <- HM₂.
+      specialize IHM₂ with E' J' (ecd E') J.
+      apply IHM₂ in HM₂; [| reflexivity | apply HJ ]. term_simpl.
+      destruct (unplug_ctrl M₂) as [[F K] |]; [| discriminate ].
+      inversion HM₂ as [[HF HK]].
+      reflexivity.
+    - destruct E'; try discriminate.
+      term_simpl in HE.
+      destruct E as [| F t' |]; try discriminate.
+      inversion HE as [[Hecd Htcd]].
+      inversion HM as [[Happ HM₂]].
+      specialize IHM₁ with E' J' (ecd E') J.
+      apply IHM₁ in Happ; [| reflexivity | apply HJ ].
+
+      remember (t_app N₁ N₂) as M₁.
+      term_simpl. destruct M₁; try discriminate; rewrite HeqM₁ in *.
+
+      rewrite Happ. reflexivity.
+    - destruct E'; try discriminate.
+      term_simpl in HE.
+      destruct E as [| F t' |]; try discriminate.
+      inversion HE as [[Hecd Htcd]].
+      inversion HM as [[Hctrl HM₂]].
+      specialize IHM₁ with E' J' (ecd E') J.
+      apply IHM₁ in Hctrl; [| reflexivity | apply HJ ].
+      term_simpl. term_simpl in Hctrl.
+      inversion Hctrl.
+      reflexivity.
+  + term_simpl.
+    destruct E'; try discriminate; subst.
+    term_simpl in HM.
+    inversion HM; subst.
+    reflexivity.
+Qed.
+
+Lemma unplug_ctrl_plug {S : VSig} (E : ectx S) J :
+  unplug_ctrl (eplug E (t_ctrl J)) = Some (ecd E, jcd J).
+Proof.
+  destruct (unplug_ctrl (eplug E (t_ctrl J))) as [[E' J'] |] eqn:Hunplug.
+  + apply unplug_ctrl_correct1 with (E' := E) (J' := J) in Hunplug as [HE HJ].
+    - rewrite HE, HJ.
+      reflexivity.
+    - reflexivity.
+  + pose proof (@unplug_ctrl_correct2 S) as Hcorrect.
+    specialize Hcorrect with (eplug E (t_ctrl J)) E J (ecd E) (jcd J).
+    destruct (Hcorrect (eq_refl (eplug E (t_ctrl J)))).
+    - reflexivity.
+    - reflexivity.
+    - symmetry. apply Hunplug.
+Qed.
+
+Lemma unplug_ctrl_some {S : VSig} (M : term S) E J :
+  unplug_ctrl M = Some (E, J) →
+  ∃ E' J', M = eplug E' (t_ctrl J') ∧ ecd E' = E ∧ jcd J' = J.
+Proof.
+  intro Hsome.
+  induction M as [ S V | S M₁ IHM₁ M₂ | S J' ].
+  + term_simpl in Hsome. discriminate.
+  + term_simpl in Hsome.
+    destruct M₁ as [ V₁ | N₁ N₂ | J₂ ].
+    - destruct (unplug_ctrl M₂) as [[F K] |]; [| discriminate ].
+      inversion Hsome as [[HF HK]].
+      specialize IHM₂ with F K.
+      destruct (IHM₂ (eq_refl (Some (F, K)))) as [F' [K' [HM₂ [Hecd Hjcd]]]].
+      exists (e_appr V₁ F'), K'.
+      repeat split.
+      * term_simpl. f_equal. apply HM₂.
+      * term_simpl. f_equal. apply Hecd.
+      * rewrite <- HK. apply Hjcd.
+    - destruct (unplug_ctrl (t_app N₁ N₂)) as [[F K] |]; [| discriminate ].
+      inversion Hsome as [[HF HK]].
+      specialize IHM₁ with F K.
+      destruct (IHM₁ (eq_refl (Some (F, K)))) as [F' [K' [Happ [Hecd Hjcd]]]].
+      exists (e_appl F' M₂), K'.
+      repeat split.
+      * term_simpl. f_equal. apply Happ.
+      * term_simpl. f_equal. apply Hecd.
+      * rewrite <- HK. apply Hjcd.
+    - term_simpl in Hsome.
+      inversion Hsome as [[HE HJ]].
+      exists (e_appl e_hole M₂), J₂.
+      repeat split.
+  + term_simpl in Hsome.
+    inversion Hsome as [[HE HJ]].
+    exists e_hole, J'.
+    repeat split.
+Qed.
+
+(* -------------------------------------------------------------------------- *)
+(* every term parallel-reduces to its complete development. *)
+
+(* In the proof of jpar_cd (below) we have a term that we know is of the form
+    M = eplug E (t_ctrl J). We then need to prove that E ⇉ₑ ecd E and J ⇉ⱼ jcd J.
+    When proving this on paper, we could just use the induction hypothesis.
+    However, Coq's termination checker won't allow that. Instead, we prove
+    that it holds for every subterm of M (subterms_cd M) and then use standalone
+    lemmas to get the desired properties. *)
+Fixpoint subterms_cd {S : VSig} (M : term S) : Prop :=
+  match M with
+  | t_app M₁ M₂ =>
+    M₁ ⇉ₜ tcd M₁
+    ∧ M₂ ⇉ₜ tcd M₂
+    ∧ subterms_cd M₁
+    ∧ subterms_cd M₂
+  | _ => True
+  end.
+
+Lemma epar_cd_plug_ind {S : VSig} (M : term S) E :
+  subterms_cd (eplug E M) →
+  E ⇉ₑ ecd E.
+Proof.
+  intros Hsubterms.
+  induction E as [| E IHE N | V E IHE ].
+  + apply epar_refl.
+  + term_simpl. term_simpl in Hsubterms.
+    destruct Hsubterms as [Hplug_cd [HN_cd [Hplug_subterms _]]].
+    constructor.
+    - apply IHE. apply Hplug_subterms.
+    - apply HN_cd.
+  + term_simpl. term_simpl in Hsubterms.
+    destruct Hsubterms as [HV_cd [Hplug_cd [_ Hplug_subterms]]].
+    constructor.
+    - apply tpar_value_invert.
+      apply HV_cd.
+    - apply IHE. apply Hplug_subterms.
+Qed.
+
+Lemma tpar_cd_plug_ind {S : VSig} (M : term S) E :
+  eplug E M ⇉ₜ tcd (eplug E M) →
+  subterms_cd (eplug E M) →
+  M ⇉ₜ tcd M.
+Proof.
+  intros HMcd Hsubterms.
+  induction E as [| E IHE N | V E IHE ].
+  + apply HMcd.
+  + term_simpl. term_simpl in Hsubterms.
+    destruct Hsubterms as [Hplug_cd [HN_cd [Hplug_subterms _]]].
+    apply IHE.
+    - apply Hplug_cd.
+    - apply Hplug_subterms.
+  + term_simpl. term_simpl in Hsubterms.
+    destruct Hsubterms as [HV_cd [Hplug_cd [_ Hplug_subterms]]].
+    apply IHE.
+    - apply Hplug_cd.
+    - apply Hplug_subterms.
+Qed.
+
+Lemma tpar_cd {S : VSig} (M : term S) :
+  M ⇉ₜ tcd M
+with vpar_cd {S : VSig} (V : value S) :
+  V ⇉ᵥ vcd V
+with jpar_cd {S : VSig} (J : jump S) :
+  J ⇉ⱼ jcd J.
+Proof.
+(* treds_cd *)
+{
+  induction M as [ ? V | A M₁ IHM₁ M₂ |].
+  + term_simpl. constructor. apply vpar_cd.
+  + term_simpl. destruct M₁ as [V | N₁ N₂ |].
+    - term_simpl. destruct V as [ x | M ].
+      * term_simpl. destruct M₂ as [ V | N₁ N₂ | J ].
+        ++ term_simpl. constructor.
+          -- apply tpar_refl.
+          -- constructor.
+            inversion IHM₂ as [| | | ? ? IHV | |]; subst.
+            apply IHV.
+        ++ constructor.
+          -- apply tpar_refl.
+          -- apply IHM₂.
+        ++ apply tpar_C_R with (V' := v_var x).
+          -- inversion IHM₂ as [| | | | | ? ? IHj ]; subst.
+            apply IHj.
+          -- apply vpar_refl.
+      * destruct M₂ as [V | N₁ N₂ | J ].
+        ++ term_simpl. constructor.
+          -- simpl in IHM₁.
+            inversion IHM₁ as [| | | ? ? IHM₁ᵥ | |]; subst.
+            inversion IHM₁ᵥ as [| ? ? IHt ]; subst.
+            apply IHt.
+          -- inversion IHM₂ as [| | | ? ? IHM₂ᵥ | |]; subst.
+            apply IHM₂ᵥ.
+        ++ constructor.
+          -- apply IHM₁.
+          -- apply IHM₂.
+        ++ constructor.
+          -- simpl in IHM₂.
+            inversion IHM₂ as [| | |  | | ? ? IHJ ]; subst.
+            apply IHJ.
+          -- inversion IHM₁; subst.
+            apply H1.
+    - constructor.
+      * apply IHM₁.
+      * apply IHM₂.
+    - constructor.
+      * inversion IHM₁ as [| | | | | ? ? IHj ]; subst.
+        apply IHj.
+      * apply IHM₂.
+  + term_simpl. constructor.
+    apply jpar_cd.
+}
+(* vpar_cd *)
+{
+  induction V as [x | M].
+  + term_simpl. apply vpar_refl.
+  + term_simpl. constructor.
+    apply tpar_cd.
+}
+(* jpar_cd *)
+{
+  induction J as [q M].
+  + term_simpl. destruct (unplug_ctrl M) as [[E J] |] eqn:Hunplug.
+    - term_simpl. apply unplug_ctrl_some in Hunplug.
+      destruct Hunplug as [E' [J' [HM [HE HJ]]]].
+
+      assert (Hsubterms: subterms_cd (eplug E' (t_ctrl J'))).
+      { rewrite <- HM.
+        clear HM HE HJ J E' J' E q.
+        induction M.
+        + term_simpl. apply I.
+        + term_simpl. repeat split.
+          - apply tpar_cd.
+          - apply tpar_cd.
+          - apply IHM1.
+          - apply IHM2.
+        + term_simpl. apply I. }
+
+      rewrite HM. constructor.
+      * rewrite <- HJ.
+
+        apply tpar_ctrl_invert.
+        apply tpar_cd_plug_ind with (M := t_ctrl J') (E := E').
+        ++ rewrite <- HM. apply tpar_cd.
+        ++ apply Hsubterms.
+      * rewrite <- HE.
+        apply epar_cd_plug_ind with (M := t_ctrl J') (E := E').
+        apply Hsubterms.
+    - constructor. apply tpar_cd.
+}
+Qed.
+
+Lemma epar_cd {S : VSig} (E : ectx S) :
+  E ⇉ₑ ecd E.
+Proof.
+  induction E; term_simpl; constructor; auto using tpar_cd, vpar_cd.
+Qed.
+
+(* -------------------------------------------------------------------------- *)
+(* ⇉ is preserved under fmap. *)
+
+Lemma tpar_map {S T : VSig} (φ : prod_arr S T) (M M' : term S) :
+  M ⇉ₜ M' →
+  fmap φ M ⇉ₜ fmap φ M'
+ with vpar_map {S T : VSig} (φ : prod_arr S T) (V V' : value S) :
+  V ⇉ᵥ V' →
+  fmap φ V ⇉ᵥ fmap φ V'
+ with jpar_map {S T : VSig} (φ : prod_arr S T) (J J' : jump S) :
+  J ⇉ⱼ J' →
+  fmap φ J ⇉ⱼ fmap φ J'
+ with epar_map {S T : VSig} (φ : prod_arr S T) (E E' : ectx S) :
+  E ⇉ₑ E' →
+  fmap φ E ⇉ₑ fmap φ E'.
+Proof.
+(* tpar_map *)
+{
+  intros Hpar.
+  generalize dependent T.
+  induction Hpar; intros T φ;
+    try (term_simpl; constructor; auto).
+  + term_simpl. rewrite fmap_struct_subst with (E := e_appl e_hole N').
+    term_simpl. constructor.
+    - apply jpar_map. apply H.
+    - apply IHHpar.
+  + term_simpl. rewrite fmap_struct_subst with (E := e_appr V' e_hole).
+    term_simpl. constructor.
+    - apply jpar_map. apply H.
+    - apply vpar_map. apply H0.
+}
+(* vpar_map *)
+{
+  intros Hpar.
+  induction Hpar;
+    try (term_simpl; constructor; auto).
+}
+(* jpar_map *)
+{
+  intros Hpar.
+  induction Hpar;
+    try (term_simpl; constructor; auto).
+  + term_simpl. rewrite eplug_fmap.
+    constructor. term_simpl.
+    - apply jpar_map. apply Hpar.
+    - apply epar_map. apply H.
+}
+(* epar_map *)
+{
+  intros Hpar.
+  induction Hpar;
+    (term_simpl; constructor; auto).
+}
+Qed.
+
+(* -------------------------------------------------------------------------- *)
+(* ⇉ is preserved under bind (substitution).
+   We use an auxiliary definition of parallel reduction for substitutions. *)
+
+Definition sspar {S : VSig} (s s' : ssub S) :=
+  let (q₁, E₁) := s  in
+  let (q₂, E₂) := s' in
+  q₁ = q₂ ∧ E₁ ⇉ₑ E₂.
+
+Notation "s ⇉ₛₛ s'" := (sspar s s') (at level 67).
+
+Lemma sspar_map {S T : VSig} (s s' : ssub S) (φ : prod_arr S T) :
+  s ⇉ₛₛ s' →
+  fmap φ s ⇉ₛₛ fmap φ s'.
+Proof.
+  intro Hpar.
+  destruct s as [q E].
+  destruct s' as [q' E'].
+  constructor.
+  + f_equal. apply Hpar.
+  + apply epar_map. apply Hpar.
+Qed.
+
+Lemma sspar_vshift {S : VSig} (s s' : ssub S) :
+  s ⇉ₛₛ s' →
+  shift (Inc := incV) s ⇉ₛₛ shift s'.
+Proof.
+  intro Hpar.
+  apply sspar_map. apply Hpar.
+Qed.
+
+Lemma sspar_kshift {S : VSig} (s s' : ssub S) :
+  s ⇉ₛₛ s' →
+  shift s ⇉ₛₛ shift s'.
+Proof.
+  intro Hpar.
+  apply sspar_map. apply Hpar.
+Qed.
+
+Lemma sspar_refl {S : VSig} (s : ssub S) :
+  s ⇉ₛₛ s.
+Proof.
+  unfold sspar.
+  destruct s; split; auto using epar_refl.
+Qed.
+
+Definition spar {S T : VSig} (φ φ' : S {→} T) :=
+  (∀ x, sub_v φ x ⇉ᵥ sub_v φ' x)
+  ∧ (∀ k, sub_k φ k ⇉ₛₛ sub_k φ' k).
+Notation "φ ⇉ₛ φ'" := (spar φ φ') (at level 67).
+
+Notation "t ↑ᵥ" := (lift (G := incV) t) (at level 15).
+
+Lemma spar_vlift {S T : VSig} (φ φ' : S {→} T) :
+  φ ⇉ₛ φ' →
+  φ ↑ᵥ ⇉ₛ φ' ↑ᵥ.
+Proof.
+  intros Hpar.
+  destruct Hpar as [Hx Hk].
+  constructor.
+  + intro x. destruct x as [| x].
+    - term_simpl. apply vpar_refl.
+    - term_simpl. apply vpar_map. apply Hx.
+  + intro k. term_simpl. apply sspar_vshift. apply Hk.
+Qed.
+
+Lemma spar_refl {S T : VSig} (φ : S {→} T) :
+  φ ⇉ₛ φ.
+Proof.
+  constructor; intro; auto using vpar_refl, sspar_refl.
+Qed.
+
+Lemma spar_klift {S T : VSig} (φ φ' : S {→} T) :
+  φ ⇉ₛ φ' →
+  φ ↑ ⇉ₛ φ' ↑.
+Proof.
+  intros Hpar.
+  destruct Hpar as [Hx Hk].
+  constructor.
+  + intro x. term_simpl. apply vpar_map. apply Hx.
+  + intro k. destruct k as [| k].
+    - term_simpl. split; [ reflexivity | apply epar_refl ].
+    - term_simpl. apply sspar_kshift. apply Hk.
+Qed.
+
+Lemma epar_comp {S : VSig} (E₂ E₂' E₁ E₁' : ectx S) :
+  E₂ ⇉ₑ E₂' →
+  E₁ ⇉ₑ E₁' →
+  ecomp E₂ E₁ ⇉ₑ ecomp E₂' E₁'.
+Proof.
+  intros Hpar₂ Hpar₁.
+  induction Hpar₂.
+  + term_simpl. apply Hpar₁.
+  + term_simpl. constructor.
+    - apply IHHpar₂. apply Hpar₁.
+    - apply H.
+  + term_simpl. constructor.
+    - apply H.
+    - apply IHHpar₂. apply Hpar₁.
+Qed.
+
+Lemma tpar_bind {S T : VSig} (M M' : term S) (φ φ' : S {→} T) :
+  φ ⇉ₛ φ' →
+  M ⇉ₜ M' →
+  bind φ M ⇉ₜ bind φ' M'
+ with vpar_bind {S T : VSig} (V V' : value S) (φ φ' : S {→} T) :
+  φ ⇉ₛ φ' →
+  V ⇉ᵥ V' →
+  bind φ V ⇉ᵥ bind φ' V'
+ with jpar_bind {S T : VSig} (J J' : jump S) (φ φ' : S {→} T) :
+  φ ⇉ₛ φ' →
+  J ⇉ⱼ J' →
+  bind φ J ⇉ⱼ bind φ' J'
+ with epar_bind {S T : VSig} (E E' : ectx S) (φ φ' : S {→} T) :
+  φ ⇉ₛ φ' →
+  E ⇉ₑ E' →
+  bind φ E ⇉ₑ bind φ' E'.
+Proof.
+(* tpar_bind *)
+{
+  intros Hφ Hpar.
+  generalize dependent T.
+  induction Hpar; intros T φ φ' Hφ.
+  + term_simpl. constructor.
+    - apply IHHpar. apply spar_vlift. apply Hφ.
+    - apply vpar_bind.
+      * apply Hφ.
+      * apply H.
+  + term_simpl.
+    rewrite bind_struct_subst with (E := e_appl e_hole N').
+    rewrite bind_liftS_shift_comm. term_simpl.
+    constructor.
+    - apply jpar_bind.
+      * apply spar_klift. apply Hφ.
+      * apply H.
+    - apply IHHpar. apply Hφ.
+  + term_simpl.
+    rewrite bind_struct_subst with (E := e_appr V' e_hole).
+    replace (e_appr (shift V) e_hole) with (shift (e_appr V e_hole)) by reflexivity.
+    term_simpl.
+    constructor.
+    - apply jpar_bind.
+      * apply spar_klift. apply Hφ.
+      * apply H.
+    - apply vpar_bind.
+      * apply Hφ.
+      * apply H0.
+  + term_simpl. constructor.
+    apply vpar_bind.
+    - apply Hφ.
+    - apply H.
+  + term_simpl. constructor.
+    - apply IHHpar1. apply Hφ.
+    - apply IHHpar2. apply Hφ.
+  + term_simpl. constructor.
+    apply jpar_bind.
+    - apply spar_klift. apply Hφ.
+    - apply H.
+}
+(* vpar_bind *)
+{
+  intros Hφ Hpar.
+  induction Hpar.
+  + term_simpl. apply Hφ.
+  + term_simpl. constructor.
+    apply tpar_bind.
+    - apply spar_vlift. apply Hφ.
+    - apply H.
+}
+(* jpar_bind *)
+{
+  intros Hφ Hpar.
+  generalize dependent T.
+  induction Hpar; intros T φ φ' Hφ.
+  + term_simpl. destruct q as [k |].
+    - pose proof Hφ as [_ Hk].
+      specialize Hk with k.
+
+      destruct (sub_k φ k) as [q F].
+      destruct (sub_k φ' k) as [q' F'].
+
+      rewrite <- eplug_bind.
+      rewrite eplug_plug_comp.
+
+      destruct Hk as [Hq HF].
+      rewrite Hq.
+
+      constructor; term_simpl.
+      * apply IHHpar. apply spar_klift. apply Hφ.
+      * apply epar_comp; [ apply HF |].
+        apply epar_bind; [ apply Hφ | apply H ].
+    - rewrite <- eplug_bind.
+      constructor; term_simpl.
+      * term_simpl. apply IHHpar. apply spar_klift. apply Hφ.
+      * apply epar_bind; [ apply Hφ | apply H ].
+  + term_simpl. destruct q as [k |].
+    - pose proof Hφ as [_ Hk].
+      specialize Hk with k.
+
+      destruct (sub_k φ k) as [q E].
+      destruct (sub_k φ' k) as [q' E'].
+
+      destruct Hk as [Hq HE].
+      rewrite Hq.
+      constructor. apply tpar_eplug; [ apply HE |].
+      apply tpar_bind; [ apply Hφ | apply H ].
+    - constructor. apply tpar_bind; [ apply Hφ | apply H ].
+}
+(* epar_bind *)
+{
+  intros Hφ Hpar.
+  induction Hpar.
+  + apply epar_refl.
+  + term_simpl. constructor.
+    - apply IHHpar. apply Hφ.
+    - apply tpar_bind; [ apply Hφ | apply H ].
+  + term_simpl. constructor.
+    - apply vpar_bind; [ apply Hφ | apply H ].
+    - apply IHHpar. apply Hφ.
+}
+Qed.
+
+Lemma spar_mk_subst_value {S : VSig} (V V' : value S) :
+  V ⇉ᵥ V' →
+  mk_subst V ⇉ₛ mk_subst V'.
+Proof.
+  intros Hpar.
+  constructor.
+  + intro x. destruct x as [| x].
+    - term_simpl. apply Hpar.
+    - term_simpl. apply vpar_refl.
+  + intro k. term_simpl. split; [ reflexivity | apply epar_refl ].
+Qed.
+
+Lemma spar_mk_subst_ectx {S : VSig} q (E E' : ectx S) :
+  E ⇉ₑ E' →
+  mk_subst (s_sub q E) ⇉ₛ mk_subst (s_sub q E').
+Proof.
+  intro Hpar.
+  constructor.
+  + intro x. term_simpl. apply vpar_refl.
+  + intro k. destruct k as [| k].
+    - term_simpl. auto.
+    - term_simpl. split.
+      * reflexivity.
+      * apply epar_refl.
+Qed.
+
+Lemma tpar_subst {S : VSig} (M M' : term (incV S)) V V' :
+  M ⇉ₜ M' →
+  V ⇉ᵥ V' →
+  subst M V ⇉ₜ subst M' V'.
+Proof.
+  intros HparM HparV.
+  apply tpar_bind.
+  + apply spar_mk_subst_value. apply HparV.
+  + apply HparM.
+Qed.
+
+Lemma spar_struct_sub {S : VSig} (E E' : ectx (incK S)) :
+  E ⇉ₑ E' →
+  struct_sub E ⇉ₛ struct_sub E'.
+Proof.
+  intro Hpar.
+  constructor.
+  + intro x. term_simpl. apply vpar_refl.
+  + intro k. destruct k as [| k].
+    - term_simpl. split; [ reflexivity | apply Hpar ].
+    - term_simpl. split; [ reflexivity | apply epar_refl ].
+Qed.
+
+Lemma jpar_struct_subst {S : VSig} (J J' : jump (incK S)) E E' :
+  J ⇉ⱼ J' →
+  E ⇉ₑ E' →
+  struct_subst J E ⇉ⱼ struct_subst J' E'.
+Proof.
+  intros HparJ HparE.
+  apply jpar_bind.
+  + apply spar_struct_sub. apply HparE.
+  + apply HparJ.
+Qed.
+
+Lemma jpar_subst {S : VSig} q (J J' : jump (incK S)) E E' :
+  J ⇉ⱼ J' →
+  E ⇉ₑ E' →
+  subst J (s_sub q E) ⇉ⱼ subst J' (s_sub q E').
+Proof.
+  intros HparJ HparE.
+  apply jpar_bind.
+  + apply spar_mk_subst_ectx. apply HparE.
+  + apply HparJ.
+Qed.
+
+(* -------------------------------------------------------------------------- *)
+(* triangle lemma:
+   if M ⇉ M', then M' ⇉ tcd M.
+      M
+     /|
+    / |
+   M' |
+    \ |
+     \|
+    tcd M
+*)
+
+Lemma tpar_eplug_invert {S : VSig} (E : ectx S) J M :
+  eplug E (t_ctrl J) ⇉ₜ M →
+  (∃ E' M', M = eplug E' M' ∧ t_ctrl J ⇉ₜ M' ∧ E ⇉ₑ E')
+  ∨ (∃ E' E'' J', M = eplug E'' (t_ctrl (struct_subst J' (shift E'))) ∧ J ⇉ⱼ J' ∧ E ⇉ₑ ecomp E'' E').
+Proof.
+  intro Hpar.
+  generalize dependent M.
+  induction E; intros M Hpar.
+  + term_simpl in Hpar.
+    inversion Hpar; subst.
+    left.
+    exists e_hole, (t_ctrl J').
+    repeat split.
+    - constructor. apply H0.
+    - apply epar_refl.
+  + term_simpl in Hpar.
+    inversion Hpar; subst.
+    - destruct E; discriminate.
+    - destruct E; try discriminate.
+      term_simpl in Hpar.
+      inversion H; subst; clear H.
+      right.
+      exists (e_appl e_hole N'), e_hole, J'.
+      repeat split.
+      * apply H1.
+      * constructor; [ apply epar_refl | apply H3 ].
+    - destruct E; discriminate.
+    - apply IHE in H1. destruct H1.
+      * destruct H as [E' [U [HM' [HJ HE]]]].
+        inversion HJ; subst.
+        left.
+        exists (e_appl E' N'), (t_ctrl J').
+        repeat split.
+        ++ constructor. apply H0.
+        ++ constructor; [ apply HE | apply H3 ].
+      * destruct H as [E' [E'' [J' [HM' [HJ HE]]]]]; subst.
+        right.
+        exists E', (e_appl E'' N'), J'.
+        repeat split.
+        ++ apply HJ.
+        ++ term_simpl. constructor; [ apply HE | apply H3 ].
+  + term_simpl in Hpar.
+    inversion Hpar; subst.
+    - destruct E; discriminate.
+    - destruct E; try discriminate.
+      inversion H0; subst; clear H0.
+      right.
+      exists (e_appr V' e_hole), e_hole, J'.
+      repeat split.
+      * apply H1.
+      * term_simpl. constructor; [ apply H3 | apply epar_refl ].
+    - apply IHE in H3. destruct H3.
+      * destruct H as [E' [U [HN' [HJ HE]]]]; subst.
+        inversion HJ; subst.
+        inversion H1; subst.
+        left.
+        exists (e_appr V' E'), (t_ctrl J').
+        repeat split.
+        ++ constructor. apply H0.
+        ++ constructor; [ apply H2 | apply HE ].
+      * destruct H as [E' [E'' [J' [HN' [HJ HE]]]]]; subst.
+        inversion H1; subst.
+        right.
+        exists E', (e_appr V' E''), J'.
+        repeat split.
+        ++ apply HJ.
+        ++ term_simpl. constructor; [ apply H0 | apply HE ].
+Qed.
+
+Lemma epar_comp_invert {S : VSig} (E E₁ E₂ : ectx S) :
+  E ⇉ₑ ecomp E₂ E₁ →
+  ∃ F₂ F₁, E = ecomp F₂ F₁ ∧ F₂ ⇉ₑ E₂ ∧ F₁ ⇉ₑ E₁.
+Proof.
+  intro Hpar.
+  generalize dependent E₁.
+  generalize dependent E₂.
+  induction E as [| E IHE M | V E IHE ]; intros E₂ E₁ Hpar.
+  + inversion Hpar.
+    destruct E₂; try discriminate.
+    destruct E₁; try discriminate.
+    exists e_hole, e_hole.
+    repeat split; apply epar_refl.
+  + inversion Hpar; subst.
+    destruct E₂; try discriminate.
+    - apply IHE with (E₂ := e_hole) in H2.
+      destruct H2 as [F₂ [F₁ [HE [HF₂ HF₁]]]].
+      inversion HF₂; subst.
+      term_simpl in H1; term_simpl; term_simpl in Hpar.
+      exists e_hole, (e_appl F₁ M).
+      repeat split.
+      * apply epar_refl.
+      * apply Hpar.
+    - term_simpl in H1.
+      inversion H1; subst.
+      apply IHE in H2.
+      destruct H2 as [F₂ [F₁ [HE [HF₂ HF₁]]]]; subst.
+      exists (e_appl F₂ M), F₁.
+      repeat split.
+      * constructor; [ apply HF₂ | apply H3 ].
+      * apply HF₁.
+  + inversion Hpar; subst.
+    destruct E₂; try discriminate.
+    - apply IHE with (E₂ := e_hole) in H3.
+      destruct H3 as [F₂ [F₁ [HE [HF₂ HF₁]]]]; subst.
+      inversion HF₂; subst.
+      term_simpl; term_simpl in H1; term_simpl in Hpar.
+      exists e_hole, (e_appr V F₁).
+      repeat split.
+      * apply epar_refl.
+      * apply Hpar.
+    - term_simpl in H1.
+      inversion H1; subst.
+      apply IHE in H3.
+      destruct H3 as [F₂ [F₁ [HE [HF₂ HF₁]]]]; subst.
+      exists (e_appr V F₂), F₁.
+      repeat split.
+      * constructor; [ apply H2 | apply HF₂ ].
+      * apply HF₁.
+Qed.
+
+Lemma ecd_ecomp {S : VSig} (E₂ E₁ : ectx S) :
+  ecd (ecomp E₂ E₁) = ecomp (ecd E₂) (ecd E₁).
+Proof.
+  induction E₂; term_simpl; f_equal; assumption.
+Qed.
+
+(* We satisfy the termination checker in a similar way as with subterms_cd. *)
+Fixpoint subterms_tcd {S : VSig} (M : term S) : Prop :=
+  match M with
+  | t_app M₁ M₂ =>
+    (∀ N₁, M₁ ⇉ₜ N₁ → N₁ ⇉ₜ tcd M₁)
+    ∧ (∀ N₂, M₂ ⇉ₜ N₂ → N₂ ⇉ₜ tcd M₂)
+    ∧ subterms_tcd M₁
+    ∧ subterms_tcd M₂
+  | _ => True
+  end.
+
+Lemma ecd_complete_plug_ind {S : VSig} (M : term S) E :
+  subterms_tcd (eplug E M) →
+  (∀ E', E ⇉ₑ E' → E' ⇉ₑ ecd E).
+Proof.
+  intro Htcd.
+  generalize dependent M.
+  induction E as [| E IHE N | V E IHE ]; intros M Htcd E' Hpar.
+  + inversion Hpar. apply epar_refl.
+  + term_simpl in Htcd.
+    destruct Htcd as [Hplug_tcd [HN_tcd [Hplug_subterms HN_subterms]]].
+    inversion Hpar as [| ? F ? N' HE HN |]; subst.
+    simpl ecd. constructor.
+    - apply IHE with M.
+      * apply Hplug_subterms.
+      * apply HE.
+    - apply HN_tcd. apply HN.
+  + term_simpl in Htcd.
+    destruct Htcd as [HV_tcd [Hplug_tcd [HV_subterms Hplug_subterms]]].
+    inversion Hpar as [| | ? V' ? F HV HE ]; subst.
+    simpl ecd. constructor.
+    - specialize HV_tcd with (t_value V').
+      apply tpar_value in HV.
+      apply HV_tcd in HV.
+      Transparent tcd.
+      inversion HV; subst.
+      apply H1.
+    - apply IHE with M.
+      * apply Hplug_subterms.
+      * apply HE.
+Qed.
+
+Lemma ecd_complete_plug_comp_ind {S : VSig} (M : term S) E₂ E₁ :
+  subterms_tcd (eplug (ecomp E₂ E₁) M) →
+  (∀ F₁, E₁ ⇉ₑ F₁ → F₁ ⇉ₑ ecd E₁)
+  ∧ (∀ F₂, E₂ ⇉ₑ F₂ → F₂ ⇉ₑ ecd E₂).
+Proof.
+  intro Htcd.
+  generalize dependent M.
+  generalize dependent E₁.
+  induction E₂ as [| E IHE N | V E IHE ]; intros E₁ M Htcd.
+  + split; intros F Hpar.
+    - apply ecd_complete_plug_ind with (E' := F) in Htcd.
+      * apply Htcd.
+      * apply Hpar.
+    - inversion Hpar. apply epar_refl.
+  + term_simpl in Htcd.
+    destruct Htcd as [Hplug_tcd [HN_tcd [Hplug_subterms HN_subterms]]].
+    apply IHE in Hplug_subterms as [HE₁ HE].
+    split.
+    - apply HE₁.
+    - intros F₂ Hpar.
+      inversion Hpar; subst.
+      term_simpl. constructor.
+      * apply HE. apply H1.
+      * apply HN_tcd. apply H3.
+  + term_simpl in Htcd.
+    destruct Htcd as [HV_tcd [Hplug_tcd [_ Hplug_subterms]]].
+    apply IHE in Hplug_subterms as [HE₁ HE].
+    split.
+    - apply HE₁.
+    - intros F₂ Hpar.
+      inversion Hpar; subst.
+      term_simpl. constructor.
+      * apply tpar_value_invert.
+        apply HV_tcd.
+        constructor. apply H1.
+      * apply HE. apply H3.
+Qed.
+
+Lemma tcd_complete_plug_ind {S : VSig} (M : term S) E :
+  (∀ M', eplug E M ⇉ₜ M' → M' ⇉ₜ tcd (eplug E M)) →
+  subterms_tcd (eplug E M) →
+  (∀ M', M ⇉ₜ M' → M' ⇉ₜ tcd M).
+Proof.
+  intros Htcd Hstcd.
+  generalize dependent M.
+  induction E as [| E IHE N | V E IHE ]; intros M Htcd Hstcd M' Hpar.
+  + apply Htcd. apply Hpar.
+  + term_simpl in Hstcd.
+    destruct Hstcd as [Hplug_tcd [HN_tcd [Hplug_subterms HN_subterms]]].
+    apply IHE.
+    - apply Hplug_tcd.
+    - apply Hplug_subterms.
+    - apply Hpar.
+  + term_simpl in Hstcd.
+    destruct Hstcd as [HV_tcd [Hplug_tcd [HV_subterms Hplug_subterms]]].
+    apply IHE.
+    - apply Hplug_tcd.
+    - apply Hplug_subterms.
+    - apply Hpar.
+Qed.
+
+Transparent tcd.
+
+Fixpoint tcd_complete {S : VSig} (M M' : term S) { struct M }:
+  M ⇉ₜ M' →
+  M' ⇉ₜ tcd M
+ with vcd_complete {S : VSig} (V V' : value S) { struct V }:
+  V ⇉ᵥ V' →
+  V' ⇉ᵥ vcd V
+ with jcd_complete {S : VSig} (J J' : jump S) { struct J }:
+  J ⇉ⱼ J' →
+  J' ⇉ⱼ jcd J.
+Proof.
+(* tcd_complete *)
+{
+  intro Hpar.
+  induction M as [ S V | S M₁ IHM₁ M₂ | S J ].
+  (* t_value V *)
+  + term_simpl. inversion Hpar as [| | | ? V' Hparᵥ | |]; subst.
+    constructor. apply vcd_complete. apply Hparᵥ.
+  (* t_app M₁ M₂ *)
+  + term_simpl. destruct M₁ as [ V | N₁ N₂ | J ].
+    (* t_app V M₂ *)
+    - destruct V as [ x | N ].
+      (* t_app (v_var x) M₂ *)
+      * destruct M₂ as [ V | N₁ N₂ | J ].
+        (* t_app (v_var x) V *)
+        ++ inversion Hpar as [| | | | ? N₁ ? N₂ HN₁ HN₂ |]; subst.
+          constructor.
+          -- apply IHM₁. apply HN₁.
+          -- apply IHM₂. apply HN₂.
+        (* t_app (v_var x) (t_app N₁ N₂) *)
+        ++ inversion Hpar as [| | | | ? U₁ ? U₂ HU₁ HU₂ |]; subst.
+          constructor.
+          -- apply IHM₁. apply HU₁.
+          -- apply IHM₂. apply HU₂.
+        (* t_app (v_var x) (t_ctrl J) *)
+        ++ inversion Hpar as [ | | ? J' ? V HJ HV | | ? M₁ ? M₂ HM₁ HM₂ |]; subst.
+          -- constructor; term_simpl.
+            apply jpar_bind.
+            ** apply spar_struct_sub.
+              constructor; [| apply epar_refl ].
+              inversion HV; subst.
+              term_simpl. apply vpar_refl.
+            ** apply jcd_complete. apply HJ.
+          -- term_simpl.
+            inversion HM₁ as [| | | ? ? HM₁ᵥ | |]; subst.
+            inversion HM₁ᵥ; subst.
+            inversion HM₂ as [| | | | | ? J' HJ ]; subst.
+            constructor 3 with (V' := v_var x).
+            ** apply jcd_complete. apply HJ.
+            ** apply vpar_refl.
+      (* t_app (v_lam N) M₂ *)
+      * destruct M₂ as [ V | N₁ N₂ | J ].
+        (* t_app (v_lam N) V *)
+        ++ term_simpl.
+          inversion Hpar as [ ? N' ? V' HN HV | | | | ? N₁ ? N₂ HN₁ HN₂ |]; subst.
+          -- apply tpar_subst.
+            ** apply tpar_lam_invert.
+              apply IHM₁.
+              constructor. constructor.
+              apply HN.
+            ** apply vcd_complete. apply HV.
+          -- inversion HN₁ as [| | | ? ? HN₁ᵥ | |]; subst.
+            inversion HN₁ᵥ as [| ? N' HN ]; subst.
+            inversion HN₂ as [| | | ? ? HN₂ᵥ | |]; subst.
+            constructor.
+            ** apply tpar_lam_invert.
+              apply IHM₁.
+              apply HN₁.
+            ** apply tpar_value_invert.
+              apply IHM₂.
+              apply HN₂.
+        (* t_app (v_lam N) (t_app N₁ N₂) *)
+        ++ inversion Hpar as [| | | | ? U₁ ? U₂ HU₁ HU₂ |]; subst.
+          constructor.
+          -- apply IHM₁. apply HU₁.
+          -- apply IHM₂. apply HU₂.
+        (* t_app (v_lam N) (t_ctrl J) *)
+        ++ inversion Hpar as [| | ? ? ? V HJ HV | | ? N₁ ? N₂ HN₁ HN₂ |]; subst.
+          -- constructor. apply jpar_struct_subst.
+            ** apply tpar_ctrl_invert.
+              apply IHM₂.
+              constructor.
+              apply HJ.
+            ** constructor; [| apply epar_refl ].
+              apply vpar_map.
+              apply tpar_value_invert.
+              apply IHM₁.
+              constructor.
+              apply HV.
+          -- inversion HN₁ as [| | | ? ? HN₁ᵥ | |]; subst.
+            inversion HN₁ᵥ as [| ? N' HN' ]; subst.
+            inversion HN₂ as [| | | | | ? J' HJ' ]; subst.
+            constructor.
+            ** apply tpar_ctrl_invert.
+              apply IHM₂.
+              apply HN₂.
+            ** apply tpar_value_invert.
+              apply IHM₁.
+              apply HN₁.
+    (* t_app (t_app N₁ N₂) M₂ *)
+    - inversion Hpar as [| | | | a1 U₁ ? U₂ HU₁ HU₂ |]; subst.
+      constructor.
+      * apply IHM₁. apply HU₁.
+      * apply IHM₂. apply HU₂.
+    (* t_app (t_ctrl J) M₂ *)
+    - inversion Hpar as [| ? J' ? M HJ HM | | | ? N₁ ? N₂ HN₁ HN₂ |]; subst.
+      * constructor.
+        apply jpar_struct_subst.
+        ++ apply tpar_ctrl_invert.
+          apply IHM₁.
+          constructor.
+          apply HJ.
+        ++ constructor; [ apply epar_refl |].
+          apply tpar_map.
+          apply IHM₂. apply HM.
+      * inversion HN₁ as [| | | | | ? J' HJ' ]; subst.
+        constructor.
+        ++ apply tpar_ctrl_invert.
+          apply IHM₁.
+          apply HN₁.
+        ++ apply IHM₂.
+          apply HN₂.
+  (* t_ctrl J *)
+  + inversion Hpar as [| | | | | ? J' HJ' ]; subst.
+    term_simpl. constructor.
+    apply jcd_complete. apply HJ'.
+}
+(* vcd_complete *)
+{
+  intro Hpar.
+  induction V as [ x | M ].
+  + inversion Hpar; subst.
+    term_simpl. apply Hpar.
+  + inversion Hpar as [| ? M' HM' ]; subst.
+    term_simpl. constructor.
+    apply tcd_complete. apply HM'.
+}
+(* jcd_complete *)
+{
+  intro Hpar.
+  induction J as [q M].
+
+  assert (Hsubterms: subterms_tcd M).
+  { clear Hpar J' q.
+    induction M.
+    + term_simpl. apply I.
+    + term_simpl.
+      repeat split.
+      - apply tcd_complete.
+      - apply tcd_complete.
+      - apply IHM1.
+      - apply IHM2.
+    + term_simpl. apply I. }
+
+  assert (IHtcd_complete: ∀ M', M ⇉ₜ M' → M' ⇉ₜ tcd M) by apply tcd_complete.
+
+  inversion Hpar; subst.
+  + term_simpl. rewrite unplug_ctrl_plug; term_simpl.
+
+    pose proof (ecd_complete_plug_ind _ _ Hsubterms) as IHecd.
+
+    apply tcd_complete_plug_ind with (M' := t_ctrl J'0) in Hsubterms as HtcdJ.
+    inversion HtcdJ; subst.
+
+    apply jpar_subst.
+    - apply H2.
+    - apply IHecd. apply H3.
+    - apply IHtcd_complete.
+    - constructor. apply H1.
+  + term_simpl. destruct (unplug_ctrl M) as [[E J] |] eqn:Hunplug.
+    - term_simpl. apply unplug_ctrl_some in Hunplug.
+      destruct Hunplug as [E' [J' [HM [Hecd Hjcd]]]].
+
+      apply tcd_complete in H2 as Htcd.
+      rewrite HM in Htcd, H2, Hsubterms, IHtcd_complete.
+
+      apply tpar_eplug_invert in H2 as Hp.
+      destruct Hp as [[F' [N' [HN' [HJ' HF']]]] | [F' [F'' [K' [HM' [HK' HF']]]]]].
+      * pose proof (ecd_complete_plug_ind _ _ Hsubterms) as IHecd.
+        inversion HJ' as [| | | | | ? K HK ]; subst.
+
+        apply tcd_complete_plug_ind with (M' := t_ctrl K) in Hsubterms as HtcdJ.
+        inversion HtcdJ; subst.
+
+        constructor.
+        ++ apply H1.
+        ++ apply IHecd. apply HF'.
+        ++ apply IHtcd_complete.
+        ++ constructor. apply HK.
+      * apply epar_comp_invert in HF'.
+        destruct HF' as [G'' [G' [HE' [HG'' HG']]]]. rewrite <- Hecd, HE'. rewrite HM'.
+
+        rewrite HE' in Hsubterms, IHtcd_complete.
+        pose proof (ecd_complete_plug_comp_ind _ _ _ Hsubterms) as [HtcdG' HtcdG''].
+
+        apply tcd_complete_plug_ind with (M' := t_ctrl K') in Hsubterms as HtcdJ.
+        inversion HtcdJ; subst.
+
+        rewrite ecd_ecomp.
+        rewrite <- subst_struct_subst.
+        constructor.
+        ++ apply jpar_struct_subst.
+          -- apply H1.
+          -- apply epar_map. apply HtcdG'. apply HG'.
+        ++ apply HtcdG''. apply HG''.
+        ++ apply IHtcd_complete.
+        ++ constructor. apply HK'.
+    - constructor. apply tcd_complete. apply H2.
+}
+Qed.
+
+(* -------------------------------------------------------------------------- *)
+(* Finally: ⇉, ⇉* and →* are confluent. *)
+
+Lemma tpar_confluence {S : VSig} (M M₁ M₂ : term S) :
+  M ⇉ₜ M₁ →
+  M ⇉ₜ M₂ →
+  ∃ M', M₁ ⇉ₜ M' ∧ M₂ ⇉ₜ M'
+ with vpar_confluence {S : VSig} (V V₁ V₂ : value S) :
+  V ⇉ᵥ V₁ →
+  V ⇉ᵥ V₂ →
+  ∃ V', V₁ ⇉ᵥ V' ∧ V₂ ⇉ᵥ V'
+ with jpar_confluence {S : VSig} (J J₁ J₂ : jump S) :
+  J ⇉ⱼ J₁ →
+  J ⇉ⱼ J₂ →
+  ∃ J', J₁ ⇉ⱼ J' ∧ J₂ ⇉ⱼ J'.
+Proof.
+(* tpar_confluence *)
+{
+  intros Hpar₁ Hpar₂.
+  exists (tcd M).
+  split; apply tcd_complete; assumption.
+}
+(* vpar_confluence *)
+{
+  intros Hpar₁ Hpar₂.
+  exists (vcd V).
+  split; apply vcd_complete; assumption.
+}
+(* jpar_confluence *)
+{
+  intros Hpar₁ Hpar₂.
+  exists (jcd J).
+  split; apply jcd_complete; assumption.
+}
+Qed.
+
+(* Auxiliary strip lemma:
+        M
+       / \
+      /   *
+     /     \
+    M₁     M₂
+     \    /
+      *  /
+       \/
+       M'
+*)
+
+Lemma tpars_strip {S : VSig} (M M₁ M₂ : term S) :
+  M ⇉ₜ M₁ →
+  M ⇉*ₜ M₂ →
+  ∃ M', M₁ ⇉*ₜ M' ∧ M₂ ⇉ₜ M'
+ with vpars_strip {S : VSig} (V V₁ V₂ : value S) :
+  V ⇉ᵥ V₁ →
+  V ⇉*ᵥ V₂ →
+  ∃ V', V₁ ⇉*ᵥ V' ∧ V₂ ⇉ᵥ V'
+ with jpars_strip {S : VSig} (J J₁ J₂ : jump S) :
+  J ⇉ⱼ J₁ →
+  J ⇉*ⱼ J₂ →
+  ∃ J', J₁ ⇉*ⱼ J' ∧ J₂ ⇉ⱼ J'.
+Proof.
+(* tpars_strip *)
+{
+  intros Hpar₁ Hpars₂.
+  generalize dependent M₁.
+  induction Hpars₂; intros M₁ Hpar₁.
+  + exists (tcd x).
+    split.
+    - constructor. apply tcd_complete. apply Hpar₁.
+    - apply tcd_complete. apply H.
+  + exists (tcd x).
+    split.
+    - constructor. apply tcd_complete. apply Hpar₁.
+    - apply tpar_cd.
+  + apply IHHpars₂1 in Hpar₁.
+    destruct Hpar₁ as [tcd₁ [HM₁ Hy]].
+    apply IHHpars₂2 in Hy.
+    destruct Hy as [tcd₂ [Htcd₁ Hz]].
+    exists (tcd₂).
+    split.
+    - constructor 3 with (y := tcd₁).
+      * apply HM₁.
+      * apply Htcd₁.
+    - apply Hz.
+}
+(* vpars_strip *)
+{
+  intros Hpar₁ Hpars₂.
+  generalize dependent V₁.
+  induction Hpars₂; intros V₁ Hpar₁.
+  + exists (vcd x).
+    split.
+    - constructor. apply vcd_complete. apply Hpar₁.
+    - apply vcd_complete. apply H.
+  + exists (vcd x).
+    split.
+    - constructor. apply vcd_complete. apply Hpar₁.
+    - apply vpar_cd.
+  + apply IHHpars₂1 in Hpar₁.
+    destruct Hpar₁ as [vcd₁ [HM₁ Hy]].
+    apply IHHpars₂2 in Hy.
+    destruct Hy as [vcd₂ [Hvcd₁ Hz]].
+    exists (vcd₂).
+    split.
+    - constructor 3 with (y := vcd₁).
+      * apply HM₁.
+      * apply Hvcd₁.
+    - apply Hz.
+}
+(* jpars_strip *)
+{
+  intros Hpar₁ Hpars₂.
+  generalize dependent J₁.
+  induction Hpars₂; intros J₁ Hpar₁.
+  + exists (jcd x).
+    split.
+    - constructor. apply jcd_complete. apply Hpar₁.
+    - apply jcd_complete. apply H.
+  + exists (jcd x).
+    split.
+    - constructor. apply jcd_complete. apply Hpar₁.
+    - apply jpar_cd.
+  + apply IHHpars₂1 in Hpar₁.
+    destruct Hpar₁ as [jcd₁ [HM₁ Hy]].
+    apply IHHpars₂2 in Hy.
+    destruct Hy as [jcd₂ [Hjcd₁ Hz]].
+    exists (jcd₂).
+    split.
+    - constructor 3 with (y := jcd₁).
+      * apply HM₁.
+      * apply Hjcd₁.
+    - apply Hz.
+}
+Qed.
+
+Lemma tpars_confluence {S : VSig} (M M₁ M₂ : term S) :
+  M ⇉*ₜ M₁ →
+  M ⇉*ₜ M₂ →
+  ∃ M', M₁ ⇉*ₜ M' ∧ M₂ ⇉*ₜ M'
+ with vpars_confluence {S : VSig} (V V₁ V₂ : value S) :
+  V ⇉*ᵥ V₁ →
+  V ⇉*ᵥ V₂ →
+  ∃ V', V₁ ⇉*ᵥ V' ∧ V₂ ⇉*ᵥ V'
+ with jpars_confluence {S : VSig} (J J₁ J₂ : jump S) :
+  J ⇉*ⱼ J₁ →
+  J ⇉*ⱼ J₂ →
+  ∃ J', J₁ ⇉*ⱼ J' ∧ J₂ ⇉*ⱼ J'.
+Proof.
+(* tpars_confluence *)
+{
+  intros Hpar₁ Hpar₂.
+  generalize dependent M₂.
+  induction Hpar₁; intros M₂ Hpar₂.
+  + pose proof (tpars_strip _ _ _ H Hpar₂) as Hstrip.
+    destruct Hstrip as [Mtcd [Hy HM₂]].
+    exists Mtcd.
+    split.
+    - apply Hy.
+    - constructor. apply HM₂.
+  + assert (Hpar₁: x ⇉ₜ x) by (apply tpar_refl).
+    pose proof (tpars_strip _ _ _ Hpar₁ Hpar₂) as Hstrip.
+    destruct Hstrip as [Mtcd [Hx HM₂]].
+    exists Mtcd.
+    split.
+    - apply Hx.
+    - constructor. apply HM₂.
+  + apply IHHpar₁1 in Hpar₂.
+    destruct Hpar₂ as [Mtcd₁ [Hy HM₂]].
+    apply IHHpar₁2 in Hy.
+    destruct Hy as [Mtcd₂ [Hz HMtcd₁]].
+    exists Mtcd₂.
+    split.
+    - apply Hz.
+    - constructor 3 with (y := Mtcd₁).
+      * apply HM₂.
+      * apply HMtcd₁.
+}
+(* vpars_confluence *)
+{
+  intros Hpar₁ Hpar₂.
+  generalize dependent V₂.
+  induction Hpar₁; intros V₂ Hpar₂.
+  + pose proof (vpars_strip _ _ _ H Hpar₂) as Hstrip.
+    destruct Hstrip as [Vvcd [Hy HV₂]].
+    exists Vvcd.
+    split.
+    - apply Hy.
+    - constructor. apply HV₂.
+  + assert (Hpar₁: x ⇉ᵥ x) by (apply vpar_refl).
+    pose proof (vpars_strip _ _ _ Hpar₁ Hpar₂) as Hstrip.
+    destruct Hstrip as [Vvcd [Hx HV₂]].
+    exists Vvcd.
+    split.
+    - apply Hx.
+    - constructor. apply HV₂.
+  + apply IHHpar₁1 in Hpar₂.
+    destruct Hpar₂ as [Vvcd₁ [Hy HV₂]].
+    apply IHHpar₁2 in Hy.
+    destruct Hy as [Vvcd₂ [Hz HVvcd₁]].
+    exists Vvcd₂.
+    split.
+    - apply Hz.
+    - constructor 3 with (y := Vvcd₁).
+      * apply HV₂.
+      * apply HVvcd₁.
+}
+(* jpars_confluence *)
+{
+  intros Hpar₁ Hpar₂.
+  generalize dependent J₂.
+  induction Hpar₁; intros J₂ Hpar₂.
+  + pose proof (jpars_strip _ _ _ H Hpar₂) as Hstrip.
+    destruct Hstrip as [Vvcd [Hy HV₂]].
+    exists Vvcd.
+    split.
+    - apply Hy.
+    - constructor. apply HV₂.
+  + assert (Hpar₁: x ⇉ⱼ x) by (apply jpar_refl).
+    pose proof (jpars_strip _ _ _ Hpar₁ Hpar₂) as Hstrip.
+    destruct Hstrip as [Vvcd [Hx HV₂]].
+    exists Vvcd.
+    split.
+    - apply Hx.
+    - constructor. apply HV₂.
+  + apply IHHpar₁1 in Hpar₂.
+    destruct Hpar₂ as [Vvcd₁ [Hy HV₂]].
+    apply IHHpar₁2 in Hy.
+    destruct Hy as [Vvcd₂ [Hz HVvcd₁]].
+    exists Vvcd₂.
+    split.
+    - apply Hz.
+    - constructor 3 with (y := Vvcd₁).
+      * apply HV₂.
+      * apply HVvcd₁.
+}
+Qed.
+
+Lemma treds_confluence {S : VSig} (M M₁ M₂ : term S) :
+  M →*ₜ M₁ →
+  M →*ₜ M₂ →
+  ∃ M', M₁ →*ₜ M' ∧ M₂ →*ₜ M'
+ with vreds_confluence {S : VSig} (V V₁ V₂ : value S) :
+  V →*ᵥ V₁ →
+  V →*ᵥ V₂ →
+  ∃ V', V₁ →*ᵥ V' ∧ V₂ →*ᵥ V'
+ with jreds_confluence {S : VSig} (J J₁ J₂ : jump S) :
+  J →*ⱼ J₁ →
+  J →*ⱼ J₂ →
+  ∃ J', J₁ →*ⱼ J' ∧ J₂ →*ⱼ J'.
+Proof.
+(* treds_confluence *)
+{
+  intros Hreds₁ Hreds₂.
+  apply treds_pars in Hreds₁.
+  apply treds_pars in Hreds₂.
+  pose proof (tpars_confluence _ _ _ Hreds₁ Hreds₂) as Hpar_conf.
+  destruct Hpar_conf as [M' [HM₁ HM₂]].
+  apply tpars_reds in HM₁.
+  apply tpars_reds in HM₂.
+  exists M'.
+  split; assumption.
+}
+(* vreds_confluence*)
+{
+  intros Hreds₁ Hreds₂.
+  apply vreds_pars in Hreds₁.
+  apply vreds_pars in Hreds₂.
+  pose proof (vpars_confluence _ _ _ Hreds₁ Hreds₂) as Hpar_conf.
+  destruct Hpar_conf as [M' [HM₁ HM₂]].
+  apply vpars_reds in HM₁.
+  apply vpars_reds in HM₂.
+  exists M'.
+  split; assumption.
+}
+(* jreds_confluence *)
+{
+  intros Hreds₁ Hreds₂.
+  apply jreds_pars in Hreds₁.
+  apply jreds_pars in Hreds₂.
+  pose proof (jpars_confluence _ _ _ Hreds₁ Hreds₂) as Hpar_conf.
+  destruct Hpar_conf as [M' [HM₁ HM₂]].
+  apply jpars_reds in HM₁.
+  apply jpars_reds in HM₂.
+  exists M'.
+  split; assumption.
+}
+Qed.
